Reworked witness-cp to allow more flexible use.
New versions of defwitness/definstantiate require unique names, so fix some books for this.

Localized some lemmas in witness-cp; fix books for this as well.

books/clause-processors/witness-cp.lisp
@@ -31,6 +31,10 @@
 (include-book "tools/def-functional-instance" :dir :system)
 (include-book "data-structures/no-duplicates" :dir :system)
 (include-book "magic-ev")
+(include-book "std/util/defaggregate" :dir :system)
+(include-book "std/util/defines" :dir :system)
+(include-book "meta-extract-user")
+(include-book "tools/easy-simplify" :dir :system)
 (set-inhibit-warnings "theory")
 
 
@@ -47,11 +51,13 @@
                            pseudo-term-list-listp nth
                            intersectp-equal-non-cons
                            substitute-into-term
-                           state-p-implies-and-forward-to-state-p1)))
+                           state-p-implies-and-forward-to-state-p1
+                           w
+                           (force))))
 
 
-;; [Jared] I localized these theorems since they're not really the point of
-;; this book, and it seems nicer not to "randomly" export stuff like this.
+;; ;; [Jared] I localized these theorems since they're not really the point of
+;; ;; this book, and it seems nicer not to "randomly" export stuff like this.
 
 (local (defthm alistp-append
          (implies (and (alistp a) (alistp b))
@@ -92,37 +98,71 @@
                        (true-listp b))
                   (equal (strip-cdrs (pairlis$ a b)) b))))
 
+(local (defthmd pseudo-term-listp-true-listp
+         (implies (pseudo-term-listp x)
+                  (true-listp x))))
+
+(local (defthmd pseudo-term-list-listp-true-listp
+         (implies (pseudo-term-list-listp x)
+                  (true-listp x))
+         :hints(("Goal" :in-theory (enable pseudo-term-list-listp)))))
+
+(local (defthmd alistp-implies-true-listp
+         (implies (alistp x) (true-listp x))
+         :hints(("Goal" :in-theory (enable alistp)))))
 
 
-(defevaluator witness-ev witness-ev-lst
-  ((if a b c) (not a) (equal a b) (use-these-hints x)
+(local (defthm pseudo-term-list-listp-append
+         (implies (and (pseudo-term-list-listp a)
+                       (pseudo-term-list-listp b))
+                  (pseudo-term-list-listp (append a b)))
+         :hints(("Goal" :in-theory (enable pseudo-term-list-listp)))))
+
+
+(local (defthm pseudo-term-listp-append
+         (implies (and (pseudo-term-listp a)
+                       (pseudo-term-listp b))
+                  (pseudo-term-listp (append a b)))
+         :hints(("Goal" :in-theory (enable pseudo-term-listp)))))
+
+(local (defthm strip-cars-of-append
+         (equal (strip-cars (append a b))
+                (append (strip-cars a) (strip-cars b)))))
+
+
+
+
+(defevaluator-fast witness-ev witness-ev-lst
+  ((if a b c)
+   (not a)
+   (equal a b)
+   (use-these-hints x)
    (implies a b) (hide x)
-   (cons a b) (binary-+ a b)))
+   (cons a b) (binary-+ a b)
+   (typespec-check ts x)
+   (iff a b))
+  :namedp t)
 
-
-(verify-termination
- (dumb-negate-lit
-  (declare
-   (xargs
-    :guard-hints(("Goal" :in-theory (enable pseudo-termp)))))))
-
-(defthm ev-dumb-negate-lit
-  (implies (pseudo-termp lit)
-           (iff (witness-ev (dumb-negate-lit lit) a)
-                (not (witness-ev lit a))))
-  :hints(("Goal" :in-theory (enable pseudo-termp))))
-
-(defthm pseudo-termp-dumb-negate-lit
-  (implies (pseudo-termp lit)
-           (pseudo-termp (dumb-negate-lit lit)))
-  :hints(("Goal" :in-theory (enable pseudo-termp
-                                    pseudo-term-listp))))
-
-(in-theory (disable dumb-negate-lit))
-
+(def-meta-extract witness-ev witness-ev-lst)
 (def-ev-theoremp witness-ev)
-
 (def-unify witness-ev witness-ev-alist)
+
+(defsection dumb-negate-lit-lemmas
+  (defthm witness-ev-of-dumb-negate-lit
+    (implies (pseudo-termp lit)
+             (iff (witness-ev (dumb-negate-lit lit) a)
+                  (not (witness-ev lit a))))
+    :hints(("Goal" :in-theory (enable pseudo-termp))))
+
+  (defthm pseudo-termp-dumb-negate-lit
+    (implies (pseudo-termp lit)
+             (pseudo-termp (dumb-negate-lit lit)))
+    :hints(("Goal" :in-theory (enable pseudo-termp
+                                      pseudo-term-listp))))
+
+  ;; non-book-local in-theory?
+  (in-theory (disable dumb-negate-lit)))
+
 
 (defun assert-msg (msg arg)
   (declare (xargs :guard t))
@@ -143,76 +183,237 @@
   `(let ((msg ,msg))
      ,(asserts-macro 'msg terms)))
 
+;;========================================================================
+;; Structures
+;;========================================================================
+
+(std::defaggregate wcp-witness-rule
+  ((name symbolp)
+   (enabledp)
+   (term pseudo-termp)
+   (expr pseudo-termp)
+   restriction
+   (theorem symbolp) ;; name of formula justifying the rule
+   (generalize (and (alistp generalize)
+                    (pseudo-term-listp (strip-cars generalize))
+                    (symbol-listp (strip-cdrs generalize))))))
+
+(std::defaggregate wcp-instance-rule
+  ((name symbolp)
+   (enabledp)
+   (pred pseudo-termp)
+   (vars (and (symbol-listp vars)
+              (not (intersectp-equal vars (simple-term-vars pred)))))
+   (expr pseudo-termp)
+   (restriction pseudo-termp)
+   (theorem symbolp)))
+
+(define wcp-instance-rulesp (x)
+  (or (atom x)
+      (and (wcp-instance-rule-p (car x))
+           (wcp-instance-rulesp (cdr x))))
+  ///
+  (defopen wcp-instance-rulesp-when-consp
+    (wcp-instance-rulesp x)
+    :hyp (consp x)
+    :hint (:expand ((wcp-instance-rulesp x)))
+    :rule-classes ((:rewrite :backchain-limit-lst 0))))
+
+(std::defaggregate wcp-template
+  ((name symbolp)
+   (enabledp)
+   (pat pseudo-termp)
+   (templ pseudo-term-listp)
+   (rulenames symbol-listp)
+   (restriction pseudo-termp)))
+
+(define wcp-templatesp (templates)
+  (or (atom templates)
+      (and (wcp-template-p (car templates))
+           (wcp-templatesp (cdr templates))))
+  ///
+  (defopen wcp-templatesp-when-consp
+    (wcp-templatesp templates)
+    :hyp (consp templates)
+    :hint (:expand ((wcp-templatesp templates)))
+    :rule-classes ((:rewrite :backchain-limit-lst 0))))
+
+(std::defaggregate wcp-example-app
+  ((instrule wcp-instance-rule-p)
+   (bindings (and (pseudo-term-listp bindings)
+                  (eql (len bindings) (len (wcp-instance-rule->vars instrule)))))))
+
+(define wcp-witness-rulesp (x)
+  (if (atom x)
+      (eq x nil)
+    (and (wcp-witness-rule-p (car x))
+         (wcp-witness-rulesp (cdr x))))
+  ///
+  (defopen wcp-witness-rulesp-when-consp
+    (wcp-witness-rulesp x)
+    :hyp (consp x)
+    :hint (:expand ((wcp-witness-rulesp x)))
+    :rule-classes ((:rewrite :backchain-limit-lst 0))))
+
+(define wcp-example-appsp (x)
+  (if (atom x)
+      (eq x nil)
+    (and (wcp-example-app-p (car x))
+         (wcp-example-appsp (cdr x))))
+  ///
+  (defopen wcp-example-appsp-when-consp
+    (wcp-example-appsp x)
+    :hyp (consp x)
+    :hint (:expand ((wcp-example-appsp x)))
+    :rule-classes ((:rewrite :backchain-limit-lst 0))))
+
+(std::defaggregate wcp-lit-actions
+  ((witnesses wcp-witness-rulesp)
+   (examples wcp-example-appsp)))
+
+(define wcp-lit-actions-listp (x)
+  (if (atom x)
+      (eq x nil)
+    (and (wcp-lit-actions-p (car x))
+         (wcp-lit-actions-listp (cdr x))))
+  ///
+  (defopen wcp-lit-actions-listp-when-consp
+    (wcp-lit-actions-listp x)
+    :hyp (consp x)
+    :hint (:expand ((wcp-lit-actions-listp x)))
+    :rule-classes ((:rewrite :backchain-limit-lst 0))))
+
+
+;; (std::defaggregate witness-cp-hints
+;;   ((generalizep)
+;;    (witness-rules wcp-witness-rulesp)
+;;    (example-templates wcp-templatesp)
+;;    (instance-rules wcp-instance-rulesp)
+;;    (examples (wcp-example-alist-listp instance-rules examples))))
+
+
 
 ;;========================================================================
-;; WITNESS-CP-EXPAND-WITNESSES
+;; WCP-MATCH-IMPLICATION
+;;========================================================================
+;; Checks that the theorem justifying a witness/instance rule is OK and
+;; therefore it's sound to apply the rule.
+
+(define wcp-match-implication ((hyp pseudo-termp)
+                               (concl pseudo-termp)
+                               (thmname symbolp)
+                               state)
+  (b* ((formula (meta-extract-formula thmname state)))
+    (and (consp formula)
+         (true-listp formula)
+         (eq (car formula) 'implies)
+         (equal (cadr formula) hyp)
+         (equal (caddr formula) concl)))
+  ///
+  (defthmd wcp-match-implication-implies
+    (implies (and (wcp-match-implication hyp concl thmname st)
+                  (witness-ev-meta-extract-global-facts)
+                  (equal (w st) (w state))
+                  (pseudo-termp hyp)
+                  (pseudo-termp concl)
+                  (witness-ev hyp a))
+             (witness-ev concl a))
+    :hints (("goal" :use ((:instance witness-ev-meta-extract-formula
+                           (name thmname)))
+             :in-theory (disable witness-ev-meta-extract-formula))))
+
+  (defthmd wcp-match-implication-implies-inv
+    (implies (and (wcp-match-implication hyp concl thmname st)
+                  (witness-ev-meta-extract-global-facts)
+                  (equal (w st) (w state))
+                  (pseudo-termp hyp)
+                  (pseudo-termp concl)
+                  (not (witness-ev concl a)))
+             (not (witness-ev hyp a)))
+    :hints (("goal" :use ((:instance witness-ev-meta-extract-formula
+                           (name thmname)))
+             :in-theory (disable witness-ev-meta-extract-formula)))))
+
+
+
+
+;;========================================================================
+;; WCP-LIT-APPLY-WITNESSES
 ;;========================================================================
 ;; (phase 1)
 
-(defun good-witness-rulesp (x)
-  (declare (Xargs :guard t))
-  (or (atom x)
-      (and (b* ((rule (car x)))
-             (asserts (msg "Failure in GOOD-WITNESS-RULESP: ~
-                            The following rule does not satisfy ~xt: ~x0.~%" rule)
-                      (true-listp rule)
-                      (equal (len rule) 7)
-                      (pseudo-termp (nth 2 rule))
-                      (pseudo-termp (nth 3 rule))
-                      (alistp (nth 6 rule))
-                      (pseudo-term-listp (strip-cars (nth 6 rule)))
-                      (symbol-listp (strip-cdrs (nth 6 rule)))))
-           (good-witness-rulesp (cdr x)))))
 
-(defun witness-generalize-alist (generalize-map alist)
-  (declare (xargs :guard (and (alistp generalize-map)
-                              (pseudo-term-listp
-                               (strip-cars generalize-map))
-                              (alistp alist))))
+
+
+(define witness-generalize-alist ((generalize-map alistp)
+                                  (alist alistp))
+  :guard (pseudo-term-listp
+          (strip-cars generalize-map))
   (pairlis$ (substitute-into-list (strip-cars generalize-map) alist)
-            (strip-cdrs generalize-map)))
+            (strip-cdrs generalize-map))
+  ///
+  (defthm alistp-witness-generalize-alist
+    (alistp (witness-generalize-alist generalize-map alist))
+    :hints(("Goal" :in-theory (enable alistp))))
 
-(defthm alistp-witness-generalize-alist
-  (alistp (witness-generalize-alist generalize-map alist))
-  :hints(("Goal" :in-theory (enable alistp))))
+  (defthm symbol-listp-cdrs-witness-generalize-alist
+    (implies (symbol-listp (strip-cdrs generalize-map))
+             (symbol-listp
+              (strip-cdrs (witness-generalize-alist generalize-map alist)))))
 
-(defthm symbol-listp-cdrs-witness-generalize-alist
-  (implies (symbol-listp (strip-cdrs generalize-map))
-           (symbol-listp
-            (strip-cdrs (witness-generalize-alist generalize-map alist)))))
+  (defthm pseudo-term-listp-cars-of-witness-generalize-alist
+    (implies (and (pseudo-term-listp (strip-cars generalize-map))
+                  (pseudo-term-val-alistp alist))
+             (pseudo-term-listp (strip-cars (witness-generalize-alist
+                                             generalize-map alist))))
+    :hints(("Goal" :in-theory (enable pseudo-term-listp)))))
 
-(in-theory (Disable witness-generalize-alist))
 
+(define wcp-lit-apply-witness ((lit pseudo-termp)
+                               (rule wcp-witness-rule-p)
+                               state)
+  :returns (mv (new-lit pseudo-term-listp :hints(("Goal" :in-theory (enable pseudo-term-listp))))
+               (genmap (and (alistp genmap)
+                            (pseudo-term-listp (strip-cars genmap))
+                            (symbol-listp (strip-cdrs genmap)))))
+  (b* (((wcp-witness-rule rule) rule)
+       ((when (not (mbt (and (wcp-witness-rule-p rule)
+                             (pseudo-termp lit)))))
+        (mv nil nil))
+       ((mv unify-ok alist)
+        (simple-one-way-unify rule.term lit nil))
+       ((when (not unify-ok))
+        (raise "Witness rule ~x0 can't be applied to literal ~x1~%" rule.name lit)
+        (mv nil nil))
+       ((unless (wcp-match-implication rule.expr rule.term rule.theorem state))
+        (raise "In witness rule ~x0, the theorem name ~x1 did not have the correct form!"
+               rule.name rule.theorem)
+        (mv nil nil))
+       (- (and (boundp-global :witness-cp-debug state)
+               (@ :witness-cp-debug)
+               (cw "Applying witness rule ~x0 to literal ~x1~%" rule.name lit)))
+       (genmap (witness-generalize-alist rule.generalize alist))
+       (new-lit (substitute-into-term rule.expr alist)))
+    (mv (list new-lit) genmap))
+  ///
+  (defthm wcp-lit-apply-witness-correct
+    (b* (((mv newlits ?gen) (wcp-lit-apply-witness lit rule st)))
+      (implies (and (not (witness-ev lit a)) ;; (not (subsetp-equal a b))
+                    (witness-ev-meta-extract-global-facts)
+                    (equal (w st) (w state)))
+               (not (witness-ev (disjoin newlits) a))))
+    :hints (("goal" 
+             :do-not-induct t
+             :in-theory (e/d (wcp-match-implication-implies)
+                             (pseudo-termp assoc-equal substitute-into-term
+                                           pseudo-term-listp
+                                           simple-one-way-unify simple-term-vars
+                                           nth))))
+    :otf-flg t))
 
-;; Witness-eval-restriction --
-;; This is an attachable function that may be used to implement arbitrary
-;; restrictions on the application of witness rules.
-;; A :restrict term may be added to witness/instance/example rules.  When
-;; attempting to apply such a rule, this term is passed to
-;; witness-eval-restriction along with the substitution alist.
-;; Witness-eval-restriction returns (mv err okp), where ERR should be an error
-;; message or NIL, and OKP says (in absence of an error) whether to apply the
-;; rule or not.
-(encapsulate
-  (((witness-eval-restriction * * state) => (mv * *)))
-  (local (defun witness-eval-restriction (term alist state)
-           (declare (xargs :stobjs state)
-                    (ignore term alist state))
-           (mv nil t))))
-
-(defun witness-eval-restriction-default (term alist state)
-  (declare (xargs :stobjs state))
-  (if (and (pseudo-termp term)
-           (symbol-alistp alist))
-      (magic-ev term (cons (cons 'world (w state)) alist)
-                state t t)
-    (mv "guards violated" nil)))
-
-(defattach witness-eval-restriction witness-eval-restriction-default)
-
-;; Lit is a member of the clause.  witness-rules is a list of tuples
+;; Lit is a member of the clause.  wcp-witness-rules is a list of tuples
 ;; conaining:
-;; rulename: name of the witness rule
+;; name: name of the witness rule
 ;; term: predicate term to match against
 ;; expr: expression implied by the predicate.
 ;; restriction: term in terms of the free vars of the predicate which
@@ -240,844 +441,184 @@
 ;;          (and (member-equal (car (set-difference-equal a b)) a)
 ;;               (not (member-equal (car (set-difference-equal a b)) b))))
 
-(defun match-lit-with-witnesses (lit witness-rules state)
-  (declare (xargs :guard (and (pseudo-termp lit)
-                              (good-witness-rulesp witness-rules))
-                  :stobjs state))
-  (b* (((when (atom witness-rules))
-        (mv nil nil nil))
-       ((when (not (mbt (pseudo-termp lit))))
-        (mv nil nil nil))
-       ((mv newlits genmap obligs)
-        (match-lit-with-witnesses lit (cdr witness-rules) state))
-       ((nths ?rulename enabledp term expr restriction hint generalize)
-        (car witness-rules))
-       ((when (not enabledp))
-        (mv newlits genmap obligs))
-       ((when (not (mbt (and (pseudo-termp term)
-                             (pseudo-termp expr)))))
-        (mv newlits genmap obligs))
+(define wcp-lit-apply-witnesses ((lit pseudo-termp)
+                                 (rules wcp-witness-rulesp)
+                                 state)
+  :returns (mv (newlits pseudo-term-listp
+                        :hints(("Goal" :in-theory (enable pseudo-term-listp pseudo-termp))))
+               (genmap (and (alistp genmap)
+                            (symbol-listp (strip-cdrs genmap))
+                            (pseudo-term-listp (strip-cars genmap)))))
+  (b* (((when (atom rules))
+        (mv nil nil))
+       ((mv newlit1 genal1)
+        (wcp-lit-apply-witness lit (car rules) state))
+       ((mv newlits genalist)
+        (wcp-lit-apply-witnesses lit (cdr rules) state)))
+    (mv (append newlit1 newlits)
+        (append genal1 genalist)))
+  ///
+  (defthm wcp-lit-apply-witnesses-correct
+    (b* (((mv newlits ?genmap) (wcp-lit-apply-witnesses lit rules st)))
+      (implies (and (not (witness-ev lit a)) ;; (not (subsetp-equal a b))
+                    (witness-ev-meta-extract-global-facts)
+                    (equal (w st) (w state)))
+               (not (witness-ev (disjoin newlits) a))))
+    :hints (("goal" :induct t))
+    :otf-flg t))
+
+
+
+;;========================================================================
+;; WCP-LIT-APPLY-EXAMPLES
+;;========================================================================
+
+(local (defthm pseudo-term-val-alistp-append
+         (implies (and (pseudo-term-val-alistp a)
+                       (pseudo-term-val-alistp b))
+                  (pseudo-term-val-alistp (append a b)))))
+
+(local
+ (defsection witness-ev-alist-lemmas
+   (defthm-simple-term-vars-flag
+     (defthm witness-ev-remove-non-var
+       (implies (and (pseudo-termp term)
+                     (not (member-equal var (simple-term-vars term))))
+                (equal (witness-ev term (cons (cons var val) a))
+                       (witness-ev term a)))
+       :flag simple-term-vars)
+     (defthm witness-ev-lst-remove-non-var
+       (implies (and (pseudo-term-listp term)
+                     (not (member-equal var (simple-term-vars-lst term))))
+                (equal (witness-ev-lst term (cons (cons var val) a))
+                       (witness-ev-lst term a)))
+       :flag simple-term-vars-lst)
+     :hints (("goal" :induct (simple-term-vars-flag flag term)
+              :in-theory (enable pseudo-termp pseudo-term-listp))
+             (and stable-under-simplificationp
+                  '(:in-theory (enable witness-ev-of-fncall-args)))))
+
+   (defthm witness-ev-remove-non-vars
+     (implies (and (pseudo-termp term)
+                   (not (intersectp-equal vars (simple-term-vars term))))
+              (equal (witness-ev term (append (pairlis$ vars vals) a))
+                     (witness-ev term a))))
+
+   (defthm witness-ev-alist-append
+     (equal (witness-ev-alist (append al1 al2) a)
+            (append (witness-ev-alist al1 a)
+                    (witness-ev-alist al2 a))))
+
+   (defthm witness-ev-alist-of-pairlis$
+     (equal (witness-ev-alist (pairlis$ keys vals) a)
+            (pairlis$ keys (witness-ev-lst vals a))))))
+
+
+(define wcp-lit-apply-example ((lit pseudo-termp)
+                               (example wcp-example-app-p)
+                               state)
+  :returns (new-lit? pseudo-term-listp :hints(("Goal" :in-theory (enable pseudo-term-listp))))
+  (b* (((unless (mbt (and (wcp-example-app-p example)
+                          (pseudo-termp lit))))
+        nil)
+       ((wcp-example-app ex) example)
+       ((wcp-instance-rule inst) ex.instrule)
        ((mv unify-ok alist)
-        (simple-one-way-unify term lit nil))
+        (simple-one-way-unify inst.pred lit nil))
        ((when (not unify-ok))
-        (mv newlits genmap obligs))
-       ((mv erp val)
-        (if (equal restriction ''t)
-            (mv nil t)
-          (witness-eval-restriction restriction alist state)))
-       ((when erp)
-        (er hard? 'match-lit-with-witnesses
-            "Evaluation of the restriction term, ~x0, produced an error: ~@1~%"
-            restriction erp)
-        (mv newlits genmap obligs))
-       ((when (not val))
-        ;; Did not conform to restriction
-        (mv newlits genmap obligs))
-       (- (and (boundp-global :witness-cp-debug state)
-               (@ :witness-cp-debug)
-               (cw "Applying witness rule ~x0~%" rulename)))
-       (genmap1 (witness-generalize-alist generalize alist))
-       (new-lit (substitute-into-term expr alist))
-       (oblig (list `(not (use-these-hints ',hint))
-                    `(implies
-                      ;; (not (subsetp-equal a b))
-                      ,(dumb-negate-lit term)
-                      ;; (and (member-equal ... a)
-                      ;;      (not (member-equal ... b)))
-                      ,(dumb-negate-lit expr)))))
-    (mv (cons new-lit newlits)
-        (append genmap1 genmap)
-        (cons oblig obligs))))
-
-(local (in-theory (Disable substitute-into-one-way-unify-reduce-list
-                           substitute-into-one-way-unify-reduce)))
-
-(defthm match-lit-with-witnesses-correct
-  (implies (not (witness-ev lit a)) ;; (not (subsetp-equal a b))
-           (mv-let (newlits rules obligs)
-             (match-lit-with-witnesses lit witness-rules state)
-             (declare (ignore rules))
-             (implies (witness-ev-theoremp
-                       (conjoin-clauses obligs))
-                      ;; (not (or (not (and (member-equal ... a)
-                      ;;                    (not (member-equal ... b))))))
-                      (not (witness-ev (disjoin newlits) a)))))
-  :hints (("goal" :induct (len witness-rules)
-           :do-not-induct t
-           :in-theory (e/d (use-these-hints)
-                           (pseudo-termp assoc-equal substitute-into-term
-                                         pseudo-term-listp
-                                         simple-one-way-unify simple-term-vars
-                                         nth)))
-          (and stable-under-simplificationp
-               '(:use ((:instance witness-ev-falsify
-                                  (x (disjoin
-                                      (car (mv-nth 2 (match-lit-with-witnesses
-                                                      lit
-                                                      witness-rules state)))))
-                                  (a (witness-ev-alist
-                                      (mv-nth 1 (simple-one-way-unify
-                                                 (nth 2 (car witness-rules))
-                                                 lit nil))
-                                      a)))))))
-  :otf-flg t)
-
-(defthm pseudo-term-listp-match-lit-with-witnesses-0
-  (pseudo-term-listp
-   (mv-nth 0 (match-lit-with-witnesses lit witness-rules state)))
-  :hints(("Goal" :in-theory (enable pseudo-term-listp pseudo-termp))))
-
-(defthm pseudo-term-list-listp-match-lit-with-witnesses-2
-  (pseudo-term-list-listp
-   (mv-nth 2 (match-lit-with-witnesses lit witness-rules state)))
-  :hints(("Goal" :in-theory (enable pseudo-term-list-listp
-                                    pseudo-term-listp
-                                    pseudo-termp))))
-
-
-(defthm alistp-match-lit-with-witnesses-1
-  (alistp
-   (mv-nth 1 (match-lit-with-witnesses lit witness-rules state))))
-
-
-(defthm symbol-listp-cdrs-match-lit-with-witnesses-1
-  (implies (good-witness-rulesp witness-rules)
-           (symbol-listp
-            (strip-cdrs
-             (mv-nth 1 (match-lit-with-witnesses lit witness-rules state))))))
-
-(in-theory (disable match-lit-with-witnesses))
-
-(defthmd pseudo-term-listp-true-listp
-  (implies (pseudo-term-listp x)
-           (true-listp x)))
-
-(defthmd pseudo-term-list-listp-true-listp
-  (implies (pseudo-term-list-listp x)
-           (true-listp x))
-  :hints(("Goal" :in-theory (enable pseudo-term-list-listp))))
-
-(defthmd alistp-implies-true-listp
-  (implies (alistp x) (true-listp x))
-  :hints(("Goal" :in-theory (enable alistp))))
-
-
-;; Transforms the clause by adding witnessing expressions and hiding the literals
-;; that generated them. Returns (mv clause rule-witness-list obligs state).
-(defun witness-cp-expand-witnesses (clause witness-rules state)
-  (declare (xargs :guard (and (pseudo-term-listp clause)
-                              (good-witness-rulesp witness-rules))
-                  :verify-guards nil
-                  :stobjs state))
-  (b* (((when (atom clause))
-        (mv nil nil nil))
-       ((mv rest genmap obligs)
-        (witness-cp-expand-witnesses (cdr clause) witness-rules state))
-       (lit (car clause))
-       ((when (not (mbt (pseudo-termp lit))))
-        (mv (cons lit rest) genmap obligs))
-       ((mv new-lits genmap1 obligs1)
-        (match-lit-with-witnesses lit witness-rules state))
-       (clause (if new-lits
-                   (cons `(not (hide ,(dumb-negate-lit lit)))
-                         (append new-lits rest))
-                 (mbe :logic (cons lit rest)
-                      :exec (if (equal rest (cdr clause))
-                                clause
-                              (cons lit rest))))))
-    (mv clause (append genmap1 genmap)
-        (append obligs1 obligs))))
-
-(verify-guards witness-cp-expand-witnesses
-               :hints (("goal" :do-not-induct t
-                        :in-theory (enable
-                                    alistp-implies-true-listp
-                                    pseudo-term-list-listp-true-listp
-                                    pseudo-term-listp
-                                    pseudo-term-listp-true-listp))))
-
-(defthm witness-cp-expand-witnesses-correct
-  (implies (not (witness-ev (disjoin clause) a))
-           (mv-let (newclause rules obligs)
-             (witness-cp-expand-witnesses clause witness-rules state)
-             (declare (ignore rules))
-             (implies (witness-ev-theoremp
-                       (conjoin-clauses obligs))
-                      ;; (not (or (not (and (member-equal ... a)
-                      ;;                    (not (member-equal ... b))))))
-                      (not (witness-ev (disjoin newclause) a)))))
-  :hints (("goal" :induct (len clause)
-           :do-not-induct t
-           :in-theory (e/d ()
-                           (pseudo-termp assoc-equal substitute-into-term
-                                         pseudo-term-listp
-                                         simple-one-way-unify simple-term-vars
-                                         nth match-lit-with-witnesses))
-           :expand ((:free (x) (hide x))))))
-
-(defthm pseudo-term-list-listp-append
-  (implies (and (pseudo-term-list-listp a)
-                (pseudo-term-list-listp b))
-           (pseudo-term-list-listp (append a b)))
-  :hints(("Goal" :in-theory (enable pseudo-term-list-listp))))
-
-
-(defthm pseudo-term-listp-append
-  (implies (and (pseudo-term-listp a)
-                (pseudo-term-listp b))
-           (pseudo-term-listp (append a b)))
-  :hints(("Goal" :in-theory (enable pseudo-term-listp))))
-
-(defthm pseudo-term-listp-witness-cp-expand-witnesses-0
-  (implies (pseudo-term-listp clause)
-           (pseudo-term-listp
-            (mv-nth 0 (witness-cp-expand-witnesses
-                       clause witness-rules state))))
-  :hints(("Goal" :in-theory (enable pseudo-term-listp
-                                    pseudo-termp))))
-
-(defthm pseudo-term-list-listp-witness-cp-expand-witnesses-2
-  (implies (pseudo-term-listp clause)
-           (pseudo-term-list-listp
-            (mv-nth 2 (witness-cp-expand-witnesses
-                       clause witness-rules state))))
-  :hints(("Goal" :in-theory (enable pseudo-term-listp))))
-
-(defthm alistp-witness-cp-expand-witnesses-1
-  (alistp (mv-nth 1 (witness-cp-expand-witnesses
-                     clause witness-rules state))))
-
-(defthm symbol-listp-cdrs-witness-cp-expand-witnesses-1
-  (implies (good-witness-rulesp witness-rules)
-           (symbol-listp
-            (strip-cdrs
-             (mv-nth 1 (witness-cp-expand-witnesses
-                        clause witness-rules state))))))
-
-(in-theory (disable witness-cp-expand-witnesses))
+        (raise "Couldn't apply instance rule ~x0 to literal ~x1~%" inst.name lit))
+       ((unless (wcp-match-implication inst.expr inst.pred inst.theorem state))
+        (raise "In instancing rule ~x0, the theorem name ~x1 did not have the correct form!"
+               inst.name inst.theorem))
+       (full-alist (append (pairlis$ inst.vars ex.bindings) alist))
+       (new-lit (substitute-into-term inst.expr full-alist)))
+    (list new-lit))
+  ///
+  (defthm wcp-lit-apply-example-correct
+    (b* ((new-lits (wcp-lit-apply-example lit example st)))
+      (implies (and (not (witness-ev lit a))
+                    (witness-ev-meta-extract-global-facts)
+                    (equal (w st) (w state)))
+               (not (witness-ev (disjoin new-lits) a))))
+    :hints(("Goal" :in-theory (enable wcp-match-implication-implies-inv)))))
 
 
 
-
-
-;;========================================================================
-;; WITNESS-CP-EXPAND-INSTANCES
-;;========================================================================
-;; (phase 3)
-
-
-(defun good-examplesp (len examples)
-  (declare (Xargs :guard t))
-  (or (atom examples)
-      (and (pseudo-term-listp (car examples))
-           (equal (len (car examples)) len)
-           (good-examplesp len (Cdr examples)))))
-
-
-(defthm alistp-pairlis$
-  (alistp (pairlis$ a b))
-  :hints(("Goal" :in-theory (enable alistp))))
-
-
-;; Vars is the list of quantified vars for the instance rule.
-;; Examples is a list of lists of expressions, each of same length as vars, to
-;; be bound to the vars.
-(defun instantiate-examples (expr vars examples alist)
-  (declare (xargs :guard (and (pseudo-termp expr)
-                              (symbol-listp vars)
-                              (good-examplesp (len vars) examples)
-                              (alistp alist))))
+(define wcp-lit-apply-examples ((lit pseudo-termp)
+                                (examples wcp-example-appsp)
+                                state)
+  :returns (new-lits pseudo-term-listp :hints(("Goal" :in-theory (enable pseudo-term-listp))))
   (if (atom examples)
       nil
-    (if (mbt (pseudo-term-listp (car examples)))
-        (cons (substitute-into-term
-               expr
-               (append (pairlis$ vars (car examples))
-                       alist))
-              (instantiate-examples expr vars (cdr examples) alist))
-      (instantiate-examples expr vars (cdr examples) alist))))
-
-(defthm pseudo-term-val-alistp-append
-  (implies (and (pseudo-term-val-alistp a)
-                (pseudo-term-val-alistp b))
-           (pseudo-term-val-alistp (append a b))))
-
-(defthm pseudo-term-listp-instantiate-examples
-  (implies (and (pseudo-termp expr)
-                (pseudo-term-val-alistp alist))
-           (pseudo-term-listp (instantiate-examples expr var examples
-                                                    alist)))
-  :hints(("Goal" :in-theory (enable pseudo-term-listp))))
-
-(defthm-simple-term-vars-flag
-  witness-ev-remove-non-var-lemma
-  (simple-term-vars
-   (implies (and (pseudo-termp term)
-                 (not (member-equal var (simple-term-vars term))))
-            (equal (witness-ev term (cons (cons var val) a))
-                   (witness-ev term a)))
-   :name witness-ev-remove-non-var)
-  (simple-term-vars-lst
-   (implies (and (pseudo-term-listp term)
-                 (not (member-equal var (simple-term-vars-lst term))))
-            (equal (witness-ev-lst term (cons (cons var val) a))
-                   (witness-ev-lst term a)))
-   :name witness-ev-lst-remove-non-var)
-  :hints (("goal" :induct (simple-term-vars-flag flag term)
-           :in-theory (enable pseudo-termp pseudo-term-listp))
-          (and stable-under-simplificationp
-               '(:in-theory (enable witness-ev-constraint-0)))))
-
-(defthm witness-ev-remove-non-vars
-  (implies (and (pseudo-termp term)
-                (not (intersectp-equal vars (simple-term-vars term))))
-           (equal (witness-ev term (append (pairlis$ vars vals) a))
-                  (witness-ev term a))))
-
-(defchoose witness-ev-satisfy-vars (vals) (term vars al)
-  (witness-ev term (append (pairlis$ vars vals) al)))
-
-(defthm witness-ev-alist-append
-  (equal (witness-ev-alist (append al1 al2) a)
-         (append (witness-ev-alist al1 a)
-                 (witness-ev-alist al2 a))))
-
-(defthm witness-ev-alist-pairlis$
-  (equal (witness-ev-alist (pairlis$ vars vals) a)
-         (pairlis$ vars (witness-ev-lst vals a))))
-
-
-(defthm instantiate-examples-correct
-  (implies (and (pseudo-termp expr)
-                (not (witness-ev expr
-                                 (append (pairlis$ vars
-                                                   (witness-ev-satisfy-vars
-                                                    expr vars (witness-ev-alist
-                                                               alist a)))
-                                       (witness-ev-alist alist a)))))
-           (not (witness-ev (disjoin (instantiate-examples expr vars examples
-                                                           alist))
-                            a)))
-  :hints (("goal" :induct (len examples))
-          (and stable-under-simplificationp
-               '(:use ((:instance witness-ev-satisfy-vars
-                                  (term expr)
-                                  (vars vars)
-                                  (vals (witness-ev-lst (car examples) a))
-                                  (al (witness-ev-alist alist
-                                                        a))))))))
-
-(in-theory (disable instantiate-examples))
-
-(defthm true-listp-union-equal
-  (equal (true-listp (union-equal a b))
-         (true-listp b))
-  :hints(("Goal" :in-theory (enable true-listp))))
-
-(defthm true-listp-simple-term-vars-lst
-  (true-listp (simple-term-vars-lst x))
-  :hints (("goal" :induct (len x)
-           :expand ((simple-term-vars-lst x)))))
-
-(defthm true-listp-simple-term-vars
-  (true-listp (simple-term-vars x))
-  :hints (("goal" :expand (simple-term-vars x))))
-
-(verify-guards simple-term-vars)
-
-;; example-alist maps each instance rulename to a list of lists of terms, each
-;; of the same length as the quantified vars of the instance rule.
-(defun good-instance-rules-and-examplesp (instance-rules example-alist)
-  (declare (xargs :guard (alistp example-alist)))
-  (b* (((when (atom instance-rules)) t)
-       (rule (car instance-rules))
-       ((when (not (true-listp rule)))
-        (cw "Not true-listp: ~x0~%" rule))
-       ((when (not (equal (len rule) 7)))
-        (cw "Wrong length: ~x0~%" rule))
-       ((nths rulename ?enabledp pred vars expr restriction ?hint) rule)
-       ((when (not (pseudo-termp pred)))
-        (cw "Not pseudo-termp: ~x0~%" pred))
-       ((when (not (pseudo-termp expr)))
-        (cw "Not pseudo-termp: ~x0~%" expr))
-       ((when (not (symbol-listp vars)))
-        (cw "Not symbol-listp: ~x0~%" vars))
-       ((when (not (symbolp rulename)))
-        (cw "Not symbolp: ~x0~%" rulename))
-       ((when (not (pseudo-termp restriction)))
-        (cw "Not pseudo-termp: ~x0~%" restriction))
-       ((when (not ;; could be intersectp
-               (not (intersectp-equal vars (simple-term-vars pred)))))
-        (cw "Intersecting vars: ~x0 ~x1~%" vars pred))
-       (look (assoc rulename example-alist))
-;;        ((when (not look))
-;;         (cw "No entry in example-alist: ~x0 ~x1~%" rulename example-alist))
-       ((when (not (good-examplesp (len vars) (cdr look))))
-        (cw "Bad examples for ~x1: ~x0~%" (cdr look) vars)))
-    (good-instance-rules-and-examplesp (cdr instance-rules) example-alist)))
-
-
-;; example-alist maps instance-rule name -> list of example expression-lists
-;; instance rules: tuple of
-;; - predicate term to match
-;; - instance-rule name
-;; - variables of example
-;; - expression implied by predicate
-;; - hint for proof oblig.
-
-;; returns: (mv new-lits obligs)
-
-(defun match-lit-with-instances (lit example-alist instance-rules state)
-  (declare (xargs :guard (and (pseudo-termp lit)
-                              (alistp example-alist)
-                              (good-instance-rules-and-examplesp
-                               instance-rules example-alist))
-                  :stobjs state))
-  (b* (((when (atom instance-rules))
-        (mv nil nil))
-       ((when (not (mbt (pseudo-termp lit))))
-        (mv nil nil))
-       ((mv newlits obligs)
-        (match-lit-with-instances
-         lit example-alist (cdr instance-rules) state))
-       ((nths rulename enabledp pred vars expr restriction hint)
-        (car instance-rules))
-       ((when (not enabledp))
-        (mv newlits obligs))
-       ((when (not (mbt (and (pseudo-termp pred)
-                             (pseudo-termp expr)
-                             (not (intersectp-equal
-                                   vars (simple-term-vars pred)))))))
-        (er hard? 'match-lit-with-instances
-            "Non pseudo-term: bad instantiate rule? ~x0~%"
-            (car instance-rules))
-        (mv newlits obligs))
-       ((mv unify-ok alist)
-        (simple-one-way-unify pred lit nil))
-       ((when (not unify-ok)) (mv newlits obligs))
-       ((mv erp val)
-        (if (equal restriction ''t)
-            (mv nil t)
-          (witness-eval-restriction restriction alist state)))
-       ((when erp)
-        (er hard? 'match-lit-with-instances
-            "Evaluation of the restriction term, ~x0, produced an error: ~@1~%"
-            restriction erp)
-        (mv newlits obligs))
-       ((when (not val))
-        ;; Did not conform to restriction
-        (mv newlits obligs))
-       (- (and (boundp-global :witness-cp-debug state)
-               (@ :witness-cp-debug)
-               (cw "Applying instance rule ~x0~%" rulename)))
-       (examples (cdr (assoc rulename example-alist)))
-       (new-lits1 (instantiate-examples expr vars examples alist))
-       (oblig (list `(not (use-these-hints ',hint))
-                    `(implies ,(dumb-negate-lit pred)
-                              ,(dumb-negate-lit expr)))))
-    (mv (append new-lits1 newlits)
-        (cons oblig obligs))))
-
-
-
-(defthm match-lit-with-instances-correct
-  (implies (not (witness-ev lit a))
-           (mv-let (newlits obligs)
-             (match-lit-with-instances lit example-alist
-                                       instance-rules state)
-             (implies (witness-ev-theoremp
-                       (conjoin-clauses obligs))
-                      (not (witness-ev (disjoin newlits) a)))))
-  :hints (("goal" :induct (len instance-rules)
-           :do-not-induct t
-           :in-theory (e/d (use-these-hints)
-                           (pseudo-termp assoc-equal substitute-into-term
-                                         pseudo-term-listp
-                                         simple-one-way-unify simple-term-vars
-                                         nth)))
-          (and stable-under-simplificationp
-               '(:use ((:instance witness-ev-falsify
-                                  (x (disjoin
-                                      (car (mv-nth 1 (match-lit-with-instances
-                                                      lit example-alist
-                                                      instance-rules state)))))
-                                  (a (append
-                                      (pairlis$ (nth 3 (car instance-rules))
-                                                (witness-ev-satisfy-vars
-                                                 (nth 4 (car instance-rules))
-                                                 (nth 3 (car instance-rules))
-                                                 (witness-ev-alist
-                                                  (mv-nth 1 (simple-one-way-unify
-                                                             (nth 2 (car instance-rules))
-                                                             lit nil))
-                                                  a)))
-                                      (witness-ev-alist
-                                       (mv-nth 1 (simple-one-way-unify
-                                                  (nth 2 (car instance-rules))
-                                                  lit nil))
-                                       a))))))))
-  :otf-flg t)
-
-
-(defthm pseudo-term-listp-match-lit-with-instances-0
-  (pseudo-term-listp
-   (mv-nth 0 (match-lit-with-instances lit example-alist
-                                       instance-rules state))))
-
-(defthm pseudo-term-list-listp-match-lit-with-instances-1
-  (pseudo-term-list-listp
-   (mv-nth 1 (match-lit-with-instances lit example-alist
-                                       instance-rules state)))
-  :hints(("Goal" :in-theory (enable pseudo-term-list-listp
-                                    pseudo-term-listp
-                                    pseudo-termp))))
-
-(in-theory (disable match-lit-with-instances))
-
-
-
-
-;; Returns (new-clause obligs).
-(defun witness-cp-expand-instances
-  (clause example-alist instance-rules state)
-  (declare (xargs :guard (and (pseudo-term-listp clause)
-                              (alistp example-alist)
-                              (good-instance-rules-and-examplesp
-                               instance-rules example-alist))
-                  :verify-guards nil
-                  :stobjs state))
-  (b* (((when (atom clause))
-        (mv nil nil))
-       ((mv rest obligs)
-        (witness-cp-expand-instances
-         (cdr clause) example-alist instance-rules state))
-       (lit (car clause))
-       ((when (not (mbt (pseudo-termp lit))))
-        (mv (cons lit rest) obligs))
-       ((mv new-lits obligs1)
-        (match-lit-with-instances lit example-alist instance-rules
-                                  state))
-       (clause (if new-lits
-                   (cons `(not (hide ,(dumb-negate-lit lit)))
-                         (append new-lits rest))
-                 (mbe :logic (cons lit rest)
-                      :exec (if (equal rest (cdr clause))
-                                clause
-                              (cons lit rest))))))
-    (mv clause (append obligs1 obligs))))
-
-(verify-guards witness-cp-expand-instances
-               :hints (("goal" :in-theory
-                        (enable pseudo-term-list-listp-true-listp
-                                pseudo-term-listp
-                                pseudo-term-listp-true-listp)
-                        :do-not-induct t)))
-
-
-(defthm witness-cp-expand-instances-correct
-  (implies (not (witness-ev (disjoin clause) a))
-           (mv-let (new-clause obligs)
-             (witness-cp-expand-instances
-              clause example-alist instance-rules state)
-             (implies (witness-ev-theoremp
-                       (conjoin-clauses obligs))
-                      (not (witness-ev (disjoin new-clause) a)))))
-  :hints (("goal" :induct (len clause)
-           :do-not-induct t
-           :in-theory (e/d ()
-                           (pseudo-termp assoc-equal substitute-into-term
-                                         pseudo-term-listp
-                                         simple-one-way-unify simple-term-vars
-                                         nth))
-           :expand ((:free (x) (hide x))))))
-
-
-(defthm pseudo-term-listp-witness-cp-expand-instances-0
-  (implies (pseudo-term-listp clause)
-           (pseudo-term-listp
-            (mv-nth 0 (witness-cp-expand-instances
-                       clause example-alist instance-rules state))))
-  :hints(("Goal" :in-theory (enable pseudo-term-listp
-                                    pseudo-termp))))
-
-
-
-(defthm pseudo-term-list-listp-witness-cp-expand-instances-2
-  (implies (pseudo-term-listp clause)
-           (pseudo-term-list-listp
-            (mv-nth 1 (witness-cp-expand-instances
-                       clause example-alist instance-rules state))))
-  :hints(("Goal" :in-theory (enable pseudo-term-listp))))
-
-
-
+    (append (wcp-lit-apply-example lit (car examples) state)
+            (wcp-lit-apply-examples lit (cdr examples) state)))
+  ///
+  (defthm wcp-lit-apply-examples-correct
+    (b* ((new-lits (wcp-lit-apply-examples lit example st)))
+      (implies (and (not (witness-ev lit a))
+                    (witness-ev-meta-extract-global-facts)
+                    (equal (w st) (w state)))
+               (not (witness-ev (disjoin new-lits) a))))))
 
 
 ;;========================================================================
-;; WITNESS-CP-COLLECT-EXAMPLES
+;; WCP-LIT-APPLY-ACTIONS
 ;;========================================================================
-;; (phase 2)
 
+(define wcp-lit-apply-actions ((lit pseudo-termp)
+                               (actions wcp-lit-actions-p)
+                               state)
+  :returns (mv (newlits pseudo-term-listp)
+               (genmap (and (alistp genmap)
+                            (symbol-listp (strip-cdrs genmap))
+                            (pseudo-term-listp (strip-cars genmap)))))
+  (b* (((mv wlits gen-alist)
+        (wcp-lit-apply-witnesses
+         lit (wcp-lit-actions->witnesses actions) state))
+       (elits
+        (wcp-lit-apply-examples
+         lit (wcp-lit-actions->examples actions) state)))
+    (mv (append wlits elits) gen-alist))
+  ///
+  (defthm wcp-lit-apply-actions-correct
+    (b* (((mv new-lits ?genalist) (wcp-lit-apply-actions lit actions st)))
+      (implies (and (not (witness-ev lit a))
+                    (witness-ev-meta-extract-global-facts)
+                    (equal (w st) (w state)))
+               (not (witness-ev (disjoin new-lits) a))))))
 
-;; (defun extract-from-alist (keys al)
-;;   (declare (xargs :guard (and (alistp al)
-;;                               (symbol-listp keys))))
-;;   (if (atom keys)
-;;       nil
-;;     (cons (cdr (assoc (car keys) al))
-;;           (extract-from-alist (cdr keys) al))))
-
-
-
-;; Example templates are of the form
-;; (term example instance-rulename)
-;; where term is the term to match,
-;; example is a list of terms using the same variables as terms,
-;; and instance-rulename is the name of the associated instance-rule.
-
-(defun good-templatesp (templates)
-  (declare (xargs :guard t))
-  (or (atom templates)
-      (let ((rule (car templates)))
-        (and (asserts
-              (msg "Failure in GOOD-TEMPLATESP: ~
-                  The following rule does not satisfy ~xt: ~x0.~%" rule)
-              (true-listp rule)
-              (equal (len rule) 6)
-              (pseudo-termp (nth 2 rule))
-              (pseudo-term-listp (nth 3 rule))
-              (symbol-listp (nth 4 rule)))
-             (good-templatesp (cdr templates))))))
-
-(defun pseudo-term-list-list-alistp (x)
-  (declare (xargs :guard t))
-  (or (atom x)
-      (and (consp (car x))
-           (pseudo-term-list-listp (cdar x))
-           (pseudo-term-list-list-alistp (cdr x)))))
-
-(defthm pseudo-term-list-list-alistp-assoc
-  (implies (pseudo-term-list-list-alistp x)
-           (pseudo-term-list-listp (cdr (assoc k x))))
-  :hints(("Goal" :in-theory (enable assoc))))
-
-(defthm pseudo-term-val-alistp-assoc
-  (implies (pseudo-term-val-alistp x)
-           (pseudo-termp (cdr (assoc k x))))
-  :hints(("Goal" :in-theory (enable assoc))))
-
-;; (defthm pseudo-term-listp-extract-from-alist
-;;   (implies (pseudo-term-val-alistp alist)
-;;            (pseudo-term-listp (extract-from-alist vars alist))))
-
-(defun add-example-for-instance-rules (inst-rules example acc)
-  (declare (xargs :guard (and (symbol-listp inst-rules)
-                              (alistp acc)
-                              (pseudo-term-listp example)
-                              (pseudo-term-list-list-alistp acc))
-                  :guard-hints (("goal" :in-theory
-                                 (enable pseudo-term-list-listp-true-listp
-                                         pseudo-term-list-listp
-                                         alistp)))))
-  (if (atom inst-rules)
-      acc
-    (b* ((rule (car inst-rules))
-         (other-examples (cdr (assoc rule acc)))
-         ((when (member-equal example other-examples))
-          (add-example-for-instance-rules (cdr inst-rules) example acc))
-         (acc (cons (cons rule (cons example other-examples)) acc)))
-      (add-example-for-instance-rules (cdr inst-rules) example acc))))
-
-(defthm pseudo-term-list-list-alistp-add-example-for-instance-rules
-  (implies (and (pseudo-term-listp example)
-                (pseudo-term-list-list-alistp acc))
-           (pseudo-term-list-list-alistp
-            (add-example-for-instance-rules
-             inst-rules example acc)))
-  :hints(("Goal" :in-theory (enable pseudo-term-list-listp))))
-
-(defthm alistp-add-example-for-instance-rules
-  (implies (alistp acc)
-           (alistp (add-example-for-instance-rules
-                    inst-rules example acc)))
-  :hints(("Goal" :in-theory (enable alistp))))
-
-
-(defun examples-for-term (term templates acc state)
-  (declare (xargs :guard (and (pseudo-termp term)
-                              (good-templatesp templates)
-                              (alistp acc)
-                              (pseudo-term-list-list-alistp acc))
-                  :verify-guards nil
-                  :stobjs state))
-  (b* (((when (atom templates)) acc)
-       ((nths ?exname enabledp pat templ rulenames restriction) (car templates))
-       ((when (not enabledp))
-        (examples-for-term term (cdr templates) acc state))
-       ((mv unify-ok alist) (simple-one-way-unify pat term nil))
-       ((when (not unify-ok))
-        (examples-for-term term (cdr templates) acc state))
-       ((mv erp val)
-        (if (equal restriction ''t)
-            (mv nil t)
-          (witness-eval-restriction restriction alist state)))
-       ((when erp)
-        (er hard? 'examples-for-term
-            "Evaluation of the restriction term, ~x0, produced an error: ~@1~%"
-            restriction erp)
-        (examples-for-term term (cdr templates) acc state))
-       ((when (not val))
-        ;; Restriction not met
-        (examples-for-term term (cdr templates) acc state))
-       (- (and (boundp-global :witness-cp-debug state)
-               (@ :witness-cp-debug)
-               (cw "Applying example rule ~x0~%" exname)))
-       (example (substitute-into-list templ alist))
-       (acc (add-example-for-instance-rules rulenames example acc)))
-    (examples-for-term term (cdr templates) acc state)))
-
-(verify-guards examples-for-term
-               :hints(("Goal" :in-theory (enable
-                                          pseudo-term-list-listp
-                                          pseudo-term-list-listp-true-listp
-                                          alistp)
-                       :do-not-induct t)))
-
-(defthm pseudo-term-list-list-alistp-examples-for-term
-  (implies (and (pseudo-termp term)
-                (good-templatesp templates)
-                (pseudo-term-list-list-alistp acc))
-           (pseudo-term-list-list-alistp
-            (examples-for-term term templates acc state)))
-  :hints(("Goal" :in-theory (enable pseudo-term-list-listp))))
-
-(defthm alistp-examples-for-term
-  (implies (alistp acc)
-           (alistp (examples-for-term term templates acc state)))
-  :hints(("Goal" :in-theory (enable alistp))))
-
-
-(in-theory (disable examples-for-term))
-
-(mutual-recursion
- (defun wcp-beta-reduce-term (x)
-   (declare (Xargs :guard (pseudo-termp x)
-                   :verify-guards nil))
-   (b* (((when (or (atom x) (eq (car X) 'quote))) x)
-        (f (car x))
-        (args (wcp-beta-reduce-list (cdr x)))
-        ((when (atom f)) (cons f args))
-        (vars (cadr f))
-        (body (wcp-beta-reduce-term (caddr f))))
-     (substitute-into-term body (pairlis$ vars args))))
- (defun wcp-beta-reduce-list (x)
-   (declare (xargs :guard (pseudo-term-listp x)))
-   (if (atom x)
-       nil
-     (cons (wcp-beta-reduce-term (car x))
-           (wcp-beta-reduce-list (cdr x))))))
-
-(flag::make-flag wcp-beta-reduce-flag wcp-beta-reduce-term)
-
-(defthm-wcp-beta-reduce-flag
-  pseudo-termp-wcp-beta-reduce-flag
-  (wcp-beta-reduce-term
-   (implies (pseudo-termp x)
-            (pseudo-termp (wcp-beta-reduce-term x)))
-   :name pseudo-termp-wcp-beta-reduce-term)
-  (wcp-beta-reduce-list
-   (implies (pseudo-term-listp x)
-            (pseudo-term-listp (wcp-beta-reduce-list x)))
-   :name pseudo-termp-wcp-beta-reduce-list)
-  :hints (("goal" :induct (wcp-beta-reduce-flag flag x)
-           :in-theory (enable pseudo-termp pseudo-term-listp))))
-
-(verify-guards wcp-beta-reduce-term
-               :hints (("goal" :in-theory (enable pseudo-termp
-                                                  pseudo-term-listp))))
-
-(mutual-recursion ;; witness-cp-collect-examples
- (defun witness-cp-collect-examples-term (x templates acc state)
-   (declare (xargs :guard (and (pseudo-termp x)
-                               (good-templatesp templates)
-                               (alistp acc)
-                               (pseudo-term-list-list-alistp acc))
-                   :verify-guards nil
-                   :stobjs state))
-   (b* (((when (atom x)) acc)
-        ((when (eq (car x) 'quote)) acc)
-        (acc
-         (witness-cp-collect-examples-list (cdr x) templates acc state))
-        ;; no lambdas -- beta reduced
-        )
-     (examples-for-term x templates acc state)))
-
- (defun witness-cp-collect-examples-list (x templates acc state)
-   (declare (xargs :guard (and (pseudo-term-listp x)
-                               (good-templatesp templates)
-                               (alistp acc)
-                               (pseudo-term-list-list-alistp acc))
-                   :stobjs state))
-   (b* (((when (atom x)) acc)
-        (acc
-         (witness-cp-collect-examples-list
-          (cdr x) templates acc state)))
-     (witness-cp-collect-examples-term
-      (car x) templates acc state))))
-
-(set-state-ok t)
-
-(flag::make-flag witness-cp-collect-examples-flag
-                 witness-cp-collect-examples-term)
-
-(defthm-witness-cp-collect-examples-flag
-  alistp-witness-cp-collect-examples
-  (witness-cp-collect-examples-term
-   (implies (alistp acc)
-            (alistp (witness-cp-collect-examples-term
-                     x templates acc state)))
-   :name alistp-witness-cp-collect-examples-term)
-  (witness-cp-collect-examples-list
-   (implies (alistp acc)
-            (alistp (witness-cp-collect-examples-list
-                     x templates acc state)))
-   :name alistp-witness-cp-collect-examples-list)
-  :hints (("goal" :induct (witness-cp-collect-examples-flag
-                           flag x templates acc state))))
-
-(defthm-witness-cp-collect-examples-flag
-  pseudo-term-list-list-alistp-witness-cp-collect-examples
-  (witness-cp-collect-examples-term
-   (implies (and (pseudo-termp x)
-                 (good-templatesp templates)
-                 (pseudo-term-list-list-alistp acc))
-            (pseudo-term-list-list-alistp
-             (witness-cp-collect-examples-term
-              x templates acc state)))
-   :name pseudo-term-list-list-alistp-witness-cp-collect-examples-term)
-  (witness-cp-collect-examples-list
-   (implies (and (pseudo-term-listp x)
-                 (good-templatesp templates)
-                 (pseudo-term-list-list-alistp acc))
-            (pseudo-term-list-list-alistp
-             (witness-cp-collect-examples-list
-              x templates acc state)))
-   :name pseudo-term-list-list-alistp-witness-cp-collect-examples-list)
-  :hints (("goal" :induct (witness-cp-collect-examples-flag
-                           flag x templates acc state)
-           :in-theory (enable pseudo-term-listp
-                              pseudo-termp))))
-
-(verify-guards witness-cp-collect-examples-term
-               :hints(("Goal" :in-theory (enable pseudo-term-listp
-                                                 pseudo-termp)
-                       :expand ((pseudo-termp x)))))
-
-
+(define wcp-clause-apply-actions ((clause pseudo-term-listp)
+                                  (actions wcp-lit-actions-listp)
+                                  state)
+  :guard (equal (len clause) (len actions))
+  :guard-hints (("goal" :in-theory (enable pseudo-term-listp
+                                           pseudo-termp)))
+  :returns (mv (new-clause pseudo-term-listp :hyp (pseudo-term-listp clause)
+                           :hints(("Goal" :in-theory (enable pseudo-term-listp
+                                                             pseudo-termp))))
+               (genmap (and (alistp genmap)
+                            (symbol-listp (strip-cdrs genmap))
+                            (pseudo-term-listp (strip-cars genmap)))))
+  (b* (((when (atom clause)) (mv nil nil))
+       ((mv first-newlits first-genalist)
+        (wcp-lit-apply-actions (car clause) (car actions) state))
+       ((mv rest-newclause rest-genalist)
+        (wcp-clause-apply-actions (cdr clause) (cdr actions) state))
+       (lit (if first-newlits `(hide ,(car clause)) (car clause))))
+    (mv (cons lit (append first-newlits rest-newclause))
+        (append first-genalist rest-genalist)))
+  ///
+  (defthm wcp-clause-apply-actions-correct
+    (b* (((mv new-clause ?genalist) (wcp-clause-apply-actions clause actions st)))
+      (implies (and (not (witness-ev (disjoin clause) a))
+                    (witness-ev-meta-extract-global-facts)
+                    (equal (w st) (w state)))
+               (not (witness-ev (disjoin new-clause) a))))
+    :hints (("goal" :expand ((:free (x) (hide x)))))))
 
 
 ;;========================================================================
-;; WITNESS-CP-GENERALIZE
+;; WCP-GENERALIZE
 ;;========================================================================
 ;; (step 4)
 
@@ -1094,630 +635,587 @@
    (gen-eval witness-ev)
    (gen-eval-lst witness-ev-lst))
   :hints((and stable-under-simplificationp
-              '(:in-theory (enable witness-ev-constraint-0)))))
+              '(:in-theory (enable witness-ev-of-fncall-args)))))
 
 
-(defun make-non-dup-vars (x avoid)
-  (declare (xargs :guard (and (symbol-listp x)
-                              (true-listp avoid))))
+(define make-non-dup-vars ((x symbol-listp)
+                           (avoid true-listp))
+  :returns (vars symbol-listp)
   (if (atom x)
       nil
     (let ((newvar (make-n-vars 1 (if (mbt (symbolp (car x)))
                                      (car x)
                                    'x) 0 avoid)))
       (append newvar
-              (make-non-dup-vars (cdr x) (append newvar avoid))))))
+              (make-non-dup-vars (cdr x) (append newvar avoid)))))
+  ///
+
+  (defthm make-non-dup-vars-not-nil
+    (not (member-equal nil (make-non-dup-vars x avoid))))
+
+  (defthm len-make-non-dup-vars
+    (equal (len (make-non-dup-vars x avoid))
+           (len x)))
+
+  (defthm no-intersect-make-non-dup-vars
+    (not (intersectp-equal avoid (make-non-dup-vars x avoid)))
+    :hints (("goal" :induct (make-non-dup-vars x avoid))
+            (and stable-under-simplificationp
+                 '(:use ((:instance make-n-vars-not-in-avoid
+                          (n 1)
+                          (base (if (symbolp (car x)) (car x) 'x)) (m 0)
+                          (avoid-lst avoid)))
+                   :in-theory (disable
+                               make-n-vars-not-in-avoid)))))
+
+  (defthm no-duplicates-make-non-dup-vars
+    (no-duplicatesp-equal (make-non-dup-vars x avoid))
+    :hints (("goal" :induct t)
+            (and stable-under-simplificationp
+                 '(:use
+                   ((:instance no-intersect-make-non-dup-vars
+                     (x (cdr x))
+                     (avoid (append
+                             (make-n-vars
+                              1 (if (symbolp (car x)) (car x)
+                                  'x)
+                              0 avoid)
+                             avoid))))
+                   :in-theory (disable
+                               no-intersect-make-non-dup-vars))))))
+
+(local
+ (defthm alistp-pairlis$
+   (alistp (pairlis$ a b))
+   :hints(("Goal" :in-theory (enable alistp)))))
 
 
-
-(defthm symbol-listp-make-non-dup-vars
-  (symbol-listp (make-non-dup-vars x avoid)))
-
-(defthm make-non-dup-vars-not-nil
-  (not (member-equal nil (make-non-dup-vars x avoid))))
-
-(defthm len-make-non-dup-vars
-  (equal (len (make-non-dup-vars x avoid))
-         (len x)))
-
-(defthm no-intersect-make-non-dup-vars
-  (not (intersectp-equal avoid (make-non-dup-vars x avoid)))
-  :hints (("goal" :induct (make-non-dup-vars x avoid))
-          (and stable-under-simplificationp
-               '(:use ((:instance make-n-vars-not-in-avoid
-                                  (n 1)
-                                  (base (if (symbolp (car x)) (car x) 'x)) (m 0)
-                                  (avoid-lst avoid)))
-                      :in-theory (disable
-                                  make-n-vars-not-in-avoid)))))
-
-(defthm no-duplicates-make-non-dup-vars
-  (no-duplicatesp-equal (make-non-dup-vars x avoid))
-  :hints (("goal" :induct t)
-          (and stable-under-simplificationp
-               '(:use
-                 ((:instance no-intersect-make-non-dup-vars
-                             (x (cdr x))
-                             (avoid (append
-                                     (make-n-vars
-                                      1 (if (symbolp (car x)) (car x)
-                                          'x)
-                                      0 avoid)
-                                     avoid))))
-                 :in-theory (disable
-                             no-intersect-make-non-dup-vars)))))
-
-(defun fix-generalize-alist (alist used-vars)
-  (declare (xargs :guard (and (alistp alist)
-                              (symbol-listp (strip-cdrs alist))
-                              (true-listp used-vars))))
+(define wcp-fix-generalize-alist ((alist (and (alistp alist)
+                                          (symbol-listp (strip-cdrs alist))))
+                              (used-vars true-listp))
+  :returns (genalist (and (alistp genalist)
+                          (not (intersectp-equal used-vars
+                                                 (strip-cdrs genalist)))
+                          (symbol-listp (strip-cdrs genalist))
+                          (not (member-equal nil (strip-cdrs genalist)))
+                          (no-duplicatesp-equal (strip-cdrs genalist)))
+                     :hints(("Goal" :in-theory (enable alistp))))
   (pairlis$ (strip-cars alist)
             (make-non-dup-vars (strip-cdrs alist) used-vars)))
 
 
-(defthm fix-generalize-alist-lemmas
-  (let ((genalist (fix-generalize-alist alist used-vars)))
-    (and (not (intersectp-equal used-vars
-                                (strip-cdrs genalist)))
-         (symbol-listp (strip-cdrs genalist))
-         (not (member-equal nil (strip-cdrs genalist)))
-         (no-duplicatesp-equal (strip-cdrs genalist)))))
 
+(define wcp-generalize-clause ((genalist (and (alistp genalist)
+                                              (symbol-listp (strip-cdrs genalist))))
+                               (clause pseudo-term-listp))
+  :prepwork ((local (defthm true-listp-make-non-dup-vars
+                      (equal (true-listp (make-non-dup-vars x avoid)) t)))
 
-(defun witness-cp-generalize-clause (genalist clause)
-  (declare (xargs :guard (and (alistp genalist)
-                              (symbol-listp (strip-cdrs genalist))
-                              (pseudo-term-listp clause))))
+             (local (defthm pseudo-term-listp-when-symbol-listp
+                      (implies (symbol-listp x)
+                               (pseudo-term-listp x))
+                      :hints (("goal" :induct (len x)
+                               :in-theory (enable symbol-listp
+                                                  pseudo-term-listp
+                                                  pseudo-termp))))))
+  :returns (newclause pseudo-term-listp
+                      :hyp (and (pseudo-term-listp clause)
+                                (alistp genalist)
+                                (symbol-listp (strip-cdrs genalist))))
   (replace-subterms-list
-   clause (fix-generalize-alist genalist
-                                (term-vars-list clause))))
+   clause (wcp-fix-generalize-alist genalist
+                                    (term-vars-list clause)))
+  ///
+  
 
+  (defthm wcp-generalize-clause-correct
+    (implies (and (bind-free '((a . a)) (a))
+                  (not (witness-ev (disjoin clause) a))
+                  (pseudo-term-listp clause))
+             (not (witness-ev-theoremp
+                   (disjoin (wcp-generalize-clause
+                             genalist clause)))))
+    :hints (("goal" :in-theory (e/d ()
+                                    (replace-subterms-list
+                                     wcp-fix-generalize-alist
+                                     term-vars-list))
+             :use ((:instance witness-ev-falsify
+                    (x (disjoin
+                        (wcp-generalize-clause
+                         genalist clause)))
+                    (a (append
+                        (witness-ev-replace-alist-to-bindings
+                         (wcp-fix-generalize-alist
+                          genalist (term-vars-list clause))
+                         a)
+                        a))))))))
 
-
-(defthm witness-cp-generalize-clause-correct
-  (implies (and (not (witness-ev-theoremp
-                      (disjoin clause)))
-                (pseudo-term-listp clause))
-           (not (witness-ev-theoremp
-                 (disjoin (witness-cp-generalize-clause
-                           genalist clause)))))
-  :hints (("goal" :in-theory (e/d ()
-                                  (replace-subterms-list
-                                   fix-generalize-alist
-                                   term-vars-list))
-           :use ((:instance witness-ev-falsify
-                            (x (disjoin
-                                (witness-cp-generalize-clause
-                                 genalist clause)))
-                            (a (append
-                                (witness-ev-replace-alist-to-bindings
-                                 (fix-generalize-alist
-                                  genalist (term-vars-list clause))
-                                 (witness-ev-falsify (disjoin clause)))
-                                (witness-ev-falsify (disjoin clause)))))))))
-
-(local (defthm true-listp-make-non-dup-vars
-         (equal (true-listp (make-non-dup-vars x avoid)) t)))
-
-
-(local (defthm pseudo-term-listp-when-symbol-listp
-         (implies (symbol-listp x)
-                  (pseudo-term-listp x))
-         :hints (("goal" :induct (len x)
-                  :in-theory (enable symbol-listp
-                                     pseudo-term-listp
-                                     pseudo-termp)))))
-
-(defthm pseudo-term-listp-witness-cp-generalize-clause
-  (implies (and (pseudo-term-listp clause)
-                (alistp genalist)
-                (symbol-listp (strip-cdrs genalist)))
-           (pseudo-term-listp
-            (witness-cp-generalize-clause genalist clause)))
-  :hints (("goal" :do-not-induct t)))
-
-(in-theory (disable witness-cp-generalize-clause))
 
 
 
 ;;========================================================================
 ;; WITNESS-CP
 ;;========================================================================
-;; (top level)
 
-;; User-provided list of examples has form:
-;;   ((instance-rulename1 term1 term2 ...)
-;;    (instance-rulename2 term1 term2 ...) ...)
-;;  --- note: not an alist, "shadowed pairs" are multiple instances of the same rule
-;; whereas we need example alist of the form
-;;   ((instance-rulename1 (term1 term2 ...) ;; example1
-;;                        (term11 term12 ...) ;; example2
-;;                        ...)
-;;    (instance-rulename2 ...))
-;;  --- note: alist, shadowed pairs ignored.
+(define witness-cp ((clause pseudo-term-listp)
+                    hint state)
+  :returns (mv err
+               (new-clause pseudo-term-list-listp
+                           :hyp (pseudo-term-listp clause)
+                           :hints(("Goal" :in-theory (enable pseudo-term-list-listp)))))
+  (b* (((unless (and (wcp-lit-actions-listp hint)
+                     (eql (len hint) (len clause))))
+        (raise "The hint to witness-cp must be a list of ~x0 objects of the ~
+                same length as the clause, which the following hint is not: ~
+                ~x1" 'wcp-lit-actions-p hint)
+        (mv nil (list clause)))
+       ((mv new-clause1 gen-alist)
+        (wcp-clause-apply-actions clause hint state)))
+    (mv nil (list (wcp-generalize-clause gen-alist new-clause1))))
+  ///
+  (defthm witness-cp-correct
+    (implies (and (pseudo-term-listp clause)
+                  (alistp a)
+                  (witness-ev-meta-extract-global-facts)
+                  (witness-ev (conjoin-clauses
+                               (clauses-result
+                                (witness-cp clause hint state)))
+                              (witness-ev-falsify
+                               (conjoin-clauses
+                                (clauses-result
+                                 (witness-cp clause hint state))))))
+             (witness-ev (disjoin clause) a))
+    :hints (("goal" :use ((:instance witness-ev-falsify
+                           (x (conjoin-clauses
+                               (clauses-result
+                                (witness-cp clause hint state))))
+                           (a a)))))
+    :rule-classes :clause-processor))
 
+(defxdoc witness-cp
+  
+  :parents (proof-automation)
+  :short "Clause processor for quantifier-based reasoning"
+  :long "<p>You should not call witness-cp directly, but rather using the
+WITNESS macro as a computed hint.  This documentation is an overview of the
+witness-cp system.</p>
 
-;; (defun pseudo-term-bindingsp (x)
-;;   ;; like LET bindings
-;;   (declare (xargs :guard t))
-;;   (if (Atom x)
-;;       (eq x nil)
-;;     (and (consp (car x))
-;;          (symbolp (caar x))
-;;          (consp (cdar x))
-;;          (pseudo-termp (cadar x))
-;;          (eq (cddar x) nil)
-;;          (pseudo-term-bindingsp (cdr x)))))
+<p>WITNESS-CP is an extensible clause processor that can use various sets of
+rules to do \"witnessing\" transformations.  Taking set-based reasoning as an
+example, we might want to look at hypotheses of the form @('(subsetp-equal a
+b)') and conclude specific examples such as @('(implies (member-equal k
+a) (member-equal k b))') for various k.  We might also want to look at
+hypotheses of the form @('(not (subsetp-equal c d))') and conclude
+@('(and (member-equal j c) (not (member-equal j d)))') for some witness
+@('j').</p>
 
-;; (local (defthm assoc-in-pseudo-term-bindingsp
-;;          (implies (and (pseudo-term-bindingsp x)
-;;                        (assoc k x))
-;;                   (and (consp (cdr (assoc k x)))
-;;                        (pseudo-termp (cadr (assoc k x)))))))
+<p>There are thus four steps to this transformation:</p>
+<ol>
+<li> Introduce witnesses for negative occurrences of universally-quantified
+ predicates and positive occurrences of existentially-quantified ones.</li>
+<li>Optionally, generalize newly introduced witness terms into fresh
+ variables, for readability.</li>
+<li> Find the set of examples with which to instantiate positive
+ universally-quantified and negative existentially-quantified predicates.</li>
+<li> Instantiate these predicates with these examples.</li>
+</ol>
 
-;; (local (defthm pseudo-term-bindingsp-implies-alistp
-;;          (implies (pseudo-term-bindingsp x)
-;;                   (alistp x))
-;;          :hints(("Goal" :in-theory (enable alistp)))))
+<p>The clause processor needs two types of information to accomplish this:</p>
+<ul>
+<li> what predicates are to be taken as universal/existential quantifiers and
+   what they mean; i.e. how to introduce witnesses/instantiate. </li>
+<li>what examples to use when doing the instantiation.</li>
+</ul>
 
-;; (local (defthm pseudo-term-bindingsp-implies-eqlable-alistp
-;;          (implies (pseudo-term-bindingsp x)
-;;                   (eqlable-alistp x))))
+<p>The witness-introduction and instantiation may both be lossy, i.e. result
+ in a formula that isn't a theorem even if the original formula is one.</p>
 
-;; (local (defthm consp-assoc
-;;          (implies (and (alistp x)
-;;                        (assoc k x))
-;;                   (consp (assoc k x)))))
+<p> To set up witnessing for not-subsetp-equal hypotheses:</p>
 
-;; (defun missing-bindings (keys bindings)
-;;   (declare (xargs :guard (pseudo-term-bindingsp bindings)))
-;;   (if (atom keys)
-;;       nil
-;;     (if (assoc (car keys) bindings)
-;;         (missing-bindings (cdr keys) bindings)
-;;       (cons (car keys)
-;;             (missing-bindings (cdr keys) bindings)))))
-
-;; (defun bindings-to-ordered-list (keys bindings)
-;;   (declare (xargs :guard (pseudo-term-bindingsp bindings)))
-;;   (if (atom keys)
-;;       nil
-;;     (cons (cdr (assoc (car keys) bindings))
-;;           (bindings-to-ordered-list (cdr keys) bindings))))
-
-
-;; just checks syntax, nothing sophisticated
-(defun good-user-examplesp (x)
-  (declare (Xargs :guard t))
-  (if (atom x)
-      (eq x nil)
-    (and (consp (car x))
-         (symbolp (caar x))
-         (pseudo-term-listp (cdar x))
-         (good-user-examplesp (cdr x)))))
-
-
-
-(defun user-examples-to-example-alist (user-examples acc)
-  (declare (xargs :guard (and (good-user-examplesp user-examples)
-                              (alistp acc)
-                              (pseudo-term-list-list-alistp acc))
-                  :guard-hints (("goal" :in-theory (enable alistp pseudo-term-list-listp)))))
-  (if (endp user-examples)
-      acc
-    (b* (((cons rulename termlist) (car user-examples))
-         (other-examples (cdr (assoc rulename acc)))
-         (acc (cons (cons rulename (cons termlist other-examples)) acc)))
-      (user-examples-to-example-alist (cdr user-examples) acc))))
-
-(defthm user-examples-to-example-alist-type
-  (let ((res (user-examples-to-example-alist user-examples acc)))
-    (and (implies (alistp acc)
-                  (alistp res))
-         (implies (and (pseudo-term-list-list-alistp acc)
-                       (good-user-examplesp user-examples))
-                  (pseudo-term-list-list-alistp res))))
-  :hints(("Goal" :in-theory (enable alistp pseudo-term-list-listp))))
-
-
-(defun witness-cp (clause hints state)
-  ":doc-section witness-cp
- witness-cp -- clause processor for quantifier-based reasoning~/
-
- You should not call witness-cp directly, but rather using the WITNESS macro
- as a computed hint.  This documentation is an overview of the witness-cp
- system.
-
- WITNESS-CP is an extensible clause processor that can use
- various sets of rules to do \"witnessing\" transformations.  Taking set-based
- reasoning as an example,  we might want to look at hypotheses of the form
- (subsetp-equal a b) and conclude specific examples such as
- (implies (member-equal k a) (member-equal k b)) for various k.  We might
- also want to look at hypotheses of the form (not (subsetp-equal c d)) and
- conclude (and (member-equal j c) (not (member-equal j d))) for some witness
- j.
-
- There are thus four steps to this transformation:
- 1. Introduce witnesses for negative occurrences of universally-quantified
- predicates and positive occurrences of existentially-quantified ones.
- 1a. Optionally, generalize newly introduced witness terms into fresh
- variables, for readability.
- 2. Find the set of examples with which to instantiate positive
- universally-quantified and negative existentially-quantified predicates.
- 3. Instantiate these predicates with these examples.
-
- The clause processor needs two types of information to accomplish this:
- - what predicates are to be taken as universal/existential quantifiers and
-   what they mean; i.e. how to introduce witnesses/instantiate.
- - what examples to use when doing the instantiation.
-
- The witness-introduction and instantiation may both be lossy, i.e. result
- in a formula that isn't a theorem even if the original formula is one.~/
-
- To set up witnessing for not-subsetp-equal hypotheses:
-
+@({
  (defwitness subsetp-witnessing
    :predicate (not (subsetp-equal a b))
    :expr (and (member-equal (subsetp-equal-witness a b) a)
               (not (member-equal (subsetp-equal-witness a b) b)))
-   :generalize (((subsetp-equal-witness a b) . ssew)
+   :generalize (((subsetp-equal-witness a b) . ssew))
    :hints ('(:in-theory '(subsetp-equal-witness-correct))))
+ })
 
- This means that in the witnessing phase, we search for hypotheses of the
+<p> This means that in the witnessing phase, we search for hypotheses of the
  form (not (subsetp-equal a b)) and for each such hypothesis, we add the
- hypothesis
+ hypothesis</p>
+@({
  (and (member-equal (subsetp-equal-witness a b) a)
       (not (member-equal (subsetp-equal-witness a b) b)))
- but then generalize away the term (subsetp-equal-witness a b) to a fresh
- variable from the set SSEW0, SSEW1, ... yielding new hyps:
+ })
+<p>but then generalize away the term (subsetp-equal-witness a b) to a fresh
+ variable from the set SSEW0, SSEW1, ... yielding new hyps:</p>
+@({
      (member-equal ssew0 a)
      (not (member-equal ssew0 b))
- So effectively we've taken an existential assumption and introduced a fresh
+ })
+<p> So effectively we've taken an existential assumption and introduced a fresh
  variable witnessing it.  We wrap (hide ...) around the original hyp to leave
  a trace of what we've done (otherwise it would likely be rewritten away,
- since the two hyps we've introduced imply its truth).
+ since the two hyps we've introduced imply its truth).</p>
 
- We add these new hypotheses to our main formula.  To ensure that this is
- sound, the clause processor produces an additional proof obligation:
+<p> We add these new hypotheses to our main formula.  To show that this is
+sound, we have the defwitness event prove the following theorem, using the
+provided hints:</p>
+@({
  (implies (not (subsetp-equal a b))
           (and (member-equal (subsetp-equal-witness a b) a)
                (not (member-equal (subsetp-equal-witness a b) b))))
- To ensure that we'll be able to satisfy this, the defwitness event tries to
- prove this using the computed hints provided by the :hint argument to
- defwitness.  In this case, this puts ACL2 into a theory containing only the
- subsetp-equal-witness-correct rule.  If the proof works, then the witness-cp
- hint will arrange for this same computed hint to be provided when the clause
- processor produces this proof obligation, and it's a fair bet that ACL2 will
- also be able to prove it then.  The hint provided is a good one because it
- puts ACL2 into a known theory (not dependent on the ambient theory); a :by
- hint is another good candidate.
+ })
 
- To set up instantiation of subsetp-equal hypotheses:
+<p>To set up instantiation of subsetp-equal hypotheses:</p>
 
+@({
  (definstantiate subsetp-equal-instancing
    :predicate (subsetp-equal a b)
    :vars (k)
    :expr (implies (member-equal k a)
                   (member-equal k b))
    :hints ('(:in-theory '(subsetp-member))))
+ })
 
- This will mean that for each subsetp-equal hypothesis we find, we'll add
+<p> This will mean that for each subsetp-equal hypothesis we find, we'll add
  hypotheses of the form (implies (member-equal k a) (member-equal k b)) for
  each of (possibly) several k.  The terms we use to instantiate k are
- determined by defexample; see below.
- To make it sound to add these hypotheses, the clause processor again
- introduces a proof obligation:
+ determined by @(see defexample); see below.
+ To show that it sound to add these hypotheses, the definstantiate event proves:</p>
+@({
   (implies (subsetp-equal a b)
            (implies (member-equal k a)
                     (member-equal k b)))
- Again, the :hints argument is used to prove this, both (as a test) when the
- definstantiate form is submitted and when it is used.
+ })
 
- The terms used to instantiate k above are determined by defexample rules,
- like the following:
+<p>The terms used to instantiate k above are determined by defexample rules,
+ like the following:</p>
+@({
   (defexample subsetp-member-template
    :pattern (member-equal k a)
    :templates (k)
    :instance-rulename subsetp-equal-instancing)
+ })
 
- This means that in phase 2, we'll look through the clause for expressions
+<p> This means that in phase 2, we'll look through the clause for expressions
  (member-equal k a) and whenever we find one, include k in the list of
  witnesses to use for instantiating using the subsetp-equal-instance rule.
  Defexample doesn't require any proof obligation; it's just a heuristic that
- adds to the set of terms used to instantiate universal quantifiers.
+ adds to the set of terms used to instantiate universal quantifiers.</p>
 
- To use the scheme we've introduced for reasoning about subsetp-equal, we can
- introduce a witness ruleset:
+<p> To use the scheme we've introduced for reasoning about subsetp-equal, we can
+ introduce a witness ruleset:</p>
 
- (def-witness-ruleset subsetp-witnessing-rules
+@({
+ (def-wcp-witness-ruleset subsetp-witnessing-rules
    '(subsetp-witnessing
      subsetp-equal-instancing
      subsetp-member-template))
+ })
 
- Then when we want to use this reasoning strategy, we can provide a computed
- hint:
+<p> Then when we want to use this reasoning strategy, we can provide a computed
+ hint:</p.
+@({
  :hints ((witness :ruleset subsetp-witnessing-rules))
+ })
 
- This implicitly waits til the formula is stable-under-simplification and
+<p> This implicitly waits til the formula is stable-under-simplification and
  invokes the witness-cp clause processor, allowing it to use the
- witnessing/instancing/example rules listed.  It also sets things up so that
- the right hints will be provided to the extra proof obligations produced by
- applying defwitness and definstantiate rules.  You can also define a macro
- so that you don't have to remember this syntax:
+ witnessing/instancing/example rules listed.  You can also define a macro
+ so that you don't have to remember this syntax:</p>
 
+@({
  (defmacro subset-reasoning () '(witness :ruleset subsetp-witnessing-rules))
  (defthm foo
    ...
   :hints ((\"goal\" ...)
           (subset-reasoning)))
+ })
 
- Documentation is available for defwitness, definstantiate, and defexample.
- Also defquantexpr, which is a shortcut for the common pattern (as above) of
- doing both a defwitness and definstantiate for a certain term.
- Also defquant, which defines a quantified function (using defun-sk) and sets
- up defwitness/definstantiate rules for it."
-  (declare (xargs :guard (pseudo-term-listp clause)
-                  :stobjs state
-                  :verify-guards nil))
-  (b* (((when (not (and (true-listp hints)
-                        (>= (len hints) 5))))
-        (er hard? 'witness-cp "Bad hints: wrong format~%")
-        (mv nil (list clause)))
-       ((nths generalizep
-              witness-rules example-templates instance-rules
-              user-examples) hints)
-       ((when (not (good-witness-rulesp witness-rules)))
-        (er hard? 'witness-cp "Bad hints: bad witness-rules~%")
-        (mv nil (list clause)))
-       ((when (not (good-templatesp example-templates)))
-        (er hard? 'witness-cp "Bad hints: bad example-templates~%")
-        (mv nil (list clause)))
-       ((when (not (good-user-examplesp user-examples)))
-        (er hard? 'witness-cp "Bad hints: bad user examples~%")
-        (mv nil (list clause)))
-       (example-alist (user-examples-to-example-alist user-examples nil))
-       ((when (not (good-instance-rules-and-examplesp
-                    instance-rules example-alist)))
-        (er hard? 'witness-cp "Bad hints: bad instance rule or user example~%")
-        (mv nil (list clause)))
-       ((mv witnessed-clause generalize-alist witness-obligs)
-        (witness-cp-expand-witnesses clause witness-rules state))
-       (generalized-clause
-        (if generalizep
-            (witness-cp-generalize-clause
-             generalize-alist witnessed-clause)
-          witnessed-clause))
-       (example-alist
-        (witness-cp-collect-examples-list
-         (wcp-beta-reduce-list generalized-clause)
-         example-templates example-alist state))
-       ((when (not (good-instance-rules-and-examplesp
-                    instance-rules example-alist)))
-        (er hard? 'witness-cp
-            "Bad hints: bad instance rule or generated example~%")
-        (mv nil (list clause)))
-       ((mv instanced-clause instance-obligs)
-        (witness-cp-expand-instances
-         generalized-clause example-alist instance-rules state))
-       ;; (generalized-clause
-       ;;  (if generalizep
-       ;;      (witness-cp-generalize-clause
-       ;;       generalize-alist instanced-clause)
-       ;;    instanced-clause))
-       )
-    (mv nil
-        (cons instanced-clause
-              (remove-duplicates-equal
-               (append instance-obligs witness-obligs))))))
-
-(verify-guards witness-cp
-               :hints (("goal" :in-theory
-                        (enable pseudo-term-list-listp-true-listp))))
-
-(defthm conjoin-clauses-remove-duplicates-equal
-  (iff (witness-ev-theoremp
-        (conjoin-clauses (remove-duplicates-equal clauses)))
-       (witness-ev-theoremp
-        (conjoin-clauses clauses))))
-
-(defthm witness-cp-correct
-  (implies (and (pseudo-term-listp clause)
-                (alistp a)
-                (witness-ev-theoremp
-                 (conjoin-clauses
-                  (clauses-result
-                   (witness-cp clause hints state)))))
-           (witness-ev (disjoin clause) a))
-  :hints(("Goal" :in-theory
-          (e/d () (good-instance-rules-and-examplesp
-                   good-witness-rulesp good-templatesp
-                   witness-cp-expand-witnesses
-                   witness-cp-collect-examples-list
-                   witness-cp-expand-instances
-                   nth len update-nth nth-0-cons nth-add1))
-          :use ((:instance witness-ev-falsify
-                           (x (disjoin clause))
-                           (a a))
-                (:instance witness-ev-falsify
-                 (x (disjoin (mv-nth 0 (witness-cp-expand-witnesses
-                                        clause (nth 1 hints) state))))
-                 (a a))
-                (:instance witness-ev-falsify
-                           (x (disjoin
-                               (car (mv-nth 1 (witness-cp clause hints state)))))
-                           (a a))
-                (:instance witness-ev-falsify
-                 (x (disjoin
-                     (car (mv-nth 1 (witness-cp clause hints state)))))
-                 (a (witness-ev-falsify
-                     (disjoin (witness-cp-generalize-clause
-                               (mv-nth 1 (witness-cp-expand-witnesses
-                                          clause (nth 1 hints) state))
-                               (mv-nth 0 (witness-cp-expand-witnesses
-                                          clause (nth 1 hints) state))))))))
-          :do-not-induct t))
-  :otf-flg t
-  :rule-classes :clause-processor)
+<p> Documentation is available for @(see defwitness), @(see definstantiate),
+and @(see defexample). Also see @(see defquantexpr), which is a shortcut for
+the common pattern (as above) of doing both a defwitness and definstantiate for
+a certain term, and @(see defquant), which defines a quantified function (using
+@(see defun-sk)) and sets up defwitness/definstantiate rules for it.</p>")
 
 
-#||
+
+;;========================================================================
+;; Heuristics for generating the hint list.
+;;========================================================================
 
 
-;; Replicate some of the proofs in equal-sets.lisp using witness-cp instead of
-;; the (set-reasoning) hint.
+;;========================================================================
+;; witness-eval-restriction
+;;========================================================================
 
-(include-book
- "equal-sets")
+;; This is an attachable function that may be used to implement arbitrary
+;; restrictions on the application of witness rules.
+;; A :restrict term may be added to witness/instance/example rules.  When
+;; attempting to apply such a rule, this term is passed to
+;; witness-eval-restriction along with the substitution alist.
+;; Witness-eval-restriction returns (mv err okp), where ERR should be an error
+;; message or NIL, and OKP says (in absence of an error) whether to apply the
+;; rule or not.
+(encapsulate
+  (((witness-eval-restriction * * state) => (mv * *)))
+  (local (defun witness-eval-restriction (term alist state)
+           (declare (xargs :stobjs state)
+                    (ignore term alist state))
+           (mv nil t))))
 
-(set-inhibit-warnings "theory")
+(defun witness-eval-restriction-default (term alist state)
+  (declare (xargs :stobjs state))
+  (if (and (pseudo-termp term)
+           (symbol-alistp alist))
+      (magic-ev term (cons (cons 'world (w state)) alist)
+                state t t)
+    (mv "guards violated" nil)))
 
-(defconst *witness-set-cp-hints*
-  '( ;; witness-rules: (pat rulename witness expr hint)
-    ((subsetp-witnessing
-      (subsetp-equal x y)
-      (subsetp-equal-witness x y)
-      (implies (member-equal (subsetp-equal-witness
-                              x y) x)
-               (member-equal (subsetp-equal-witness
-                              x y) y))
-      ('(:in-theory (e/d
-                     (subsetp-equal-witness-correct)
-                     (subsetp-equal
-                      member-equal)))))
-     (intersectp-equal-witnessing
-      (not (intersectp-equal x y))
-      (intersectp-equal-witness x y)
-      (not (if (member-equal (intersectp-equal-witness
-                              x y) x)
-               (member-equal (intersectp-equal-witness
-                              x y) y)
-             'nil))
-      ('(:in-theory (e/d
-                     (intersectp-equal-witness-correct)
-                     (intersectp-equal
-                      member-equal)))))
-     (consp-witnessing
-      (not (consp x))
-      (car x)
-      (not (member-equal (car x) x))
-      ('(:in-theory (enable member-equal)))))
-    ;; example templates: (pat vars rulename)
-    (((member-equal k y)
-      (k)
-      intersectp-equal-instancing)
-     ((member-equal k y)
-      (k)
-      subsetp-equal-instancing)
-     ((member-equal k y)
-      (k)
-      consp-instancing))
-; instance-rules: (pat rulename vars expr hint)
-    ((subsetp-equal-instancing
-      (not (subsetp-equal x y))
-      (k)
-      (not (implies (member-equal k x)
-                    (member-equal k y)))
-      ('(:in-theory (e/d (subsetp-member)
-                         (subsetp-equal
-                          member-equal)))))
-     (intersectp-equal-instancing
-      (intersectp-equal x y)
-      (k)
-      (if (member-equal k x)
-          (member-equal k y)
-        'nil)
-      ('(:in-theory (e/d (intersectp-equal-member)
-                         (intersectp-equal
-                          member-equal)))))
-     (consp-instancing
-      (consp x)
-      (k)
-      (member-equal k x)
-      ('(:in-theory (enable member-equal)))))))
-
-(defthm intersectp-equal-iff-intersection-equal2
-  (iff (consp (intersection-equal x y))
-       (intersectp-equal x y))
-  :hints (("Goal" :do-not-induct t)
-          (and stable-under-simplificationp
-               '(:computed-hint-replacement
-                 ((use-these-hints-hint clause))
-                 :clause-processor
-                 (witness-cp clause
-                             *witness-set-cp-hints*))))
-  :otf-flg t
-  :rule-classes nil)
-
-(defthm intersectp-of-superset-2
-  (implies (and (intersectp-equal a b)
-                (subsetp-equal a c))
-           (intersectp-equal c b))
-  :hints (("Goal" :do-not-induct t)
-          (and stable-under-simplificationp
-               '(:computed-hint-replacement
-                 ((use-these-hints-hint clause))
-                 :clause-processor
-                 (witness-cp clause
-                             *witness-set-cp-hints*))))
-  :otf-flg t
-  :rule-classes nil)
-
-(defthm intersectp-of-superset2-2
-  (implies (and (subsetp-equal a c)
-                (intersectp-equal b a))
-           (intersectp-equal b c))
-  :hints (("Goal" :do-not-induct t)
-          (and stable-under-simplificationp
-               '(:computed-hint-replacement
-                 ((use-these-hints-hint clause))
-                 :clause-processor
-                 (witness-cp clause
-                             *witness-set-cp-hints*))))
-  :otf-flg t
-  :rule-classes nil)
-
-(defthm subsetp-equal-cons-same-2
-  (implies (subsetp-equal a b)
-           (subsetp-equal (cons x a) (cons x b)))
-  :hints (("Goal" :do-not-induct t
-           :in-theory (disable subsetp-equal-cons-same))
-          (and stable-under-simplificationp
-               '(:computed-hint-replacement
-                 ((use-these-hints-hint clause))
-                 :clause-processor
-                 (witness-cp clause
-                             *witness-set-cp-hints*))))
-  :otf-flg t
-  :rule-classes nil)
+(defattach witness-eval-restriction witness-eval-restriction-default)
 
 
 
 
-||#
+(define wcp-witnesses-for-lit ((lit pseudo-termp)
+                               (witness-rules wcp-witness-rulesp)
+                               state)
+  :returns (rules wcp-witness-rulesp)
+  (b* (((when (atom witness-rules))
+        nil)
+       (rest (wcp-witnesses-for-lit lit (cdr witness-rules) state))
+       ((unless (mbt (wcp-witness-rule-p (car witness-rules)))) rest)
+       ((wcp-witness-rule rule) (car witness-rules))
+       ((mv unify-ok alist)
+        (simple-one-way-unify rule.term lit nil))
+       ((unless unify-ok) rest)
+       ((mv erp val)
+        (if (equal rule.restriction ''t)
+            (mv nil t)
+          (witness-eval-restriction rule.restriction alist state)))
+       ((when erp)
+        (raise
+         "Evaluation of the restriction term, ~x0, produced an error: ~@1~%"
+         rule.restriction erp)
+        rest)
+       ((when (not val)) rest))
+    (cons (car witness-rules) rest)))
 
 
-;; Keep the various kinds of rules in a table.
-;; Witness rules:     witness-cp-witness-rules
-;; Example templates: witness-cp-example-templates
-;; Instance rules:    witness-cp-instance-rules.
+(define wcp-find-instance-rule ((name symbolp)
+                                (inst-rules wcp-instance-rulesp))
+  :returns (rule (iff (wcp-instance-rule-p rule) rule))
+  (if (atom inst-rules)
+      nil
+    (if (and (mbt (wcp-instance-rule-p (car inst-rules)))
+             (eq (wcp-instance-rule->name (car inst-rules)) name))
+        (car inst-rules)
+      (wcp-find-instance-rule name (cdr inst-rules)))))
 
-;; Another table, witness-cp-rulesets, will be used to store subsets
-;; of these rules.
+(define wcp-add-example-apps ((bindings pseudo-term-listp)
+                              (inst-rulenames symbol-listp)
+                              (inst-rules wcp-instance-rulesp)
+                              (acc wcp-example-appsp))
+  :returns (apps wcp-example-appsp
+                 :hyp (wcp-example-appsp acc))
+  (b* (((when (atom inst-rulenames)) acc)
+       (rule (wcp-find-instance-rule (car inst-rulenames) inst-rules))
+       (rest (wcp-add-example-apps bindings (cdr inst-rulenames) inst-rules acc))
+       ((unless (and rule
+                     (mbt (pseudo-term-listp bindings))
+                     (eql (len (wcp-instance-rule->vars rule))
+                          (len bindings))))
+        rest))
+    (cons (make-wcp-example-app :instrule rule :bindings bindings)
+          rest)))
 
-(defun run-test-with-hint-replacement (term hints ctx state)
-  (declare (xargs :mode :program :stobjs state))
-  (with-ctx-summarized
-    ctx
-    (b* (((er hint)
-          (translate-hints+ 'thm '((use-these-hints-hint clause))
-                            nil 'ctx (w state) state))
-         (clauses `(((not (use-these-hints ',hints))
-                     ,term)))
-         (pspv (make-pspv (ens state) (w state) :orig-hints hint
-                          :displayed-goal term))
-         ((er ttree)
-          (prove-loop clauses pspv hint (ens state) (w state) ctx state)))
-      (chk-assumption-free-ttree ttree ctx state))))
+
+(define wcp-examples-for-term ((term pseudo-termp)
+                               (templates wcp-templatesp)
+                               (inst-rules wcp-instance-rulesp)
+                               (acc wcp-example-appsp)
+                               state)
+  :returns (exalist wcp-example-appsp
+                    :hyp (wcp-example-appsp acc))
+  (b* (((when (atom templates)) acc)
+       ((unless (mbt (and (wcp-template-p (car templates))
+                          (pseudo-termp term))))
+        (wcp-examples-for-term term (cdr templates) inst-rules acc state))
+       ((wcp-template tmpl) (car templates))
+;; (nths ?exname enabledp pat templ rulenames restriction)
+       ((when (not tmpl.enabledp))
+        (wcp-examples-for-term term (cdr templates) inst-rules acc state))
+       ((mv unify-ok alist) (simple-one-way-unify tmpl.pat term nil))
+       ((when (not unify-ok))
+        (wcp-examples-for-term term (cdr templates) inst-rules acc state))
+       ((mv erp val)
+        (if (equal tmpl.restriction ''t)
+            (mv nil t)
+          (witness-eval-restriction tmpl.restriction alist state)))
+       ((when erp)
+        (raise
+         "Evaluation of the restriction term, ~x0, produced an error: ~@1~%"
+         tmpl.restriction erp)
+        (wcp-examples-for-term term (cdr templates) inst-rules acc state))
+       ((when (not val))
+        ;; Restriction not met
+        (wcp-examples-for-term term (cdr templates) inst-rules acc state))
+       (bindings (substitute-into-list tmpl.templ alist))
+       (acc (wcp-add-example-apps bindings tmpl.rulenames inst-rules acc)))
+    (wcp-examples-for-term term (cdr templates) inst-rules acc state)))
+
+(std::defines wcp-beta-reduce
+  :verify-guards nil
+  (define wcp-beta-reduce-term ((x pseudo-termp))
+    :returns (res pseudo-termp :hyp (pseudo-termp x)
+                  :hints ('(:in-theory (enable pseudo-termp))))
+    :flag term
+    (b* (((when (or (atom x) (eq (car X) 'quote))) x)
+         (f (car x))
+         (args (wcp-beta-reduce-list (cdr x)))
+         ((when (atom f)) (cons f args))
+         (vars (cadr f))
+         (body (wcp-beta-reduce-term (caddr f))))
+      (substitute-into-term body (pairlis$ vars args))))
+  (define wcp-beta-reduce-list ((x pseudo-term-listp))
+    :returns (res pseudo-term-listp :hyp (pseudo-term-listp x)
+                  :hints('(:in-theory (enable pseudo-term-listp))))
+    :flag list
+    (if (atom x)
+        nil
+      (cons (wcp-beta-reduce-term (car x))
+            (wcp-beta-reduce-list (cdr x)))))
+  ///
+
+  (verify-guards wcp-beta-reduce-term
+    :hints (("goal" :in-theory (enable pseudo-termp
+                                       pseudo-term-listp)))))
+
+
+(set-state-ok t)
+
+(std::defines wcp-collect-examples
+  :verify-guards nil
+  (define wcp-collect-examples-term ((x pseudo-termp)
+                                            (templates wcp-templatesp)
+                                            (inst-rules wcp-instance-rulesp)
+                                            (acc wcp-example-appsp)
+                                            state)
+    :returns (res wcp-example-appsp
+                  :hyp (wcp-example-appsp acc))
+    :flag term
+    (b* (((when (atom x)) acc)
+         ((when (eq (car x) 'quote)) acc)
+         (acc
+          (wcp-collect-examples-list (cdr x) templates inst-rules acc state))
+         ;; no lambdas -- beta reduced
+         )
+      (wcp-examples-for-term x templates inst-rules acc state)))
+
+  (define wcp-collect-examples-list ((x pseudo-term-listp)
+                                            (templates wcp-templatesp)
+                                            (inst-rules wcp-instance-rulesp)
+                                            (acc wcp-example-appsp)
+                                            state)
+    :returns (res wcp-example-appsp
+                  :hyp (wcp-example-appsp acc))
+    :flag list
+    (b* (((when (atom x)) acc)
+         (acc
+          (wcp-collect-examples-list
+           (cdr x) templates inst-rules acc state)))
+      (wcp-collect-examples-term
+       (car x) templates inst-rules acc state)))
+  ///
+  (verify-guards wcp-collect-examples-term
+    :hints(("Goal" :expand ((pseudo-termp x)
+                            (pseudo-term-listp x))))))
+
+
+(define wcp-example-apps-for-lit ((lit pseudo-termp)
+                                  (examples wcp-example-appsp)
+                                  state)
+  :returns (apps wcp-example-appsp)
+  (b* (((when (atom examples)) nil)
+       (rest (wcp-example-apps-for-lit lit (cdr examples) state))
+       ((when (not (mbt (wcp-example-app-p (car examples))))) rest)
+       ((wcp-example-app ex) (car examples))
+       ((wcp-instance-rule rule) ex.instrule)
+       ((when (not rule.enabledp)) rest)
+       ((mv unify-ok alist)
+        (simple-one-way-unify rule.pred lit nil))
+       ((when (not unify-ok)) rest)
+       ((mv erp val)
+        (if (equal rule.restriction ''t)
+            (mv nil t)
+          (witness-eval-restriction rule.restriction alist state)))
+       ((when erp)
+        (raise "Evaluation of the restriction term, ~x0, produced an error: ~@1~%"
+               rule.restriction erp)
+        rest)
+       ((when (not val))
+        ;; Did not conform to restriction
+        rest))
+    (cons (car examples) rest)))
+
+(define wcp-lit-actions-for-lit ((lit pseudo-termp)
+                                 (examples wcp-example-appsp)
+                                 (witness-rules wcp-witness-rulesp)
+                                 state)
+  :returns (actions wcp-lit-actions-p)
+  (make-wcp-lit-actions
+   :witnesses (wcp-witnesses-for-lit lit witness-rules state)
+   :examples (wcp-example-apps-for-lit lit examples state)))
+
+
+
+(define wcp-actions-for-lits ((lits pseudo-term-listp)
+                              (examples wcp-example-appsp)
+                              (witness-rules wcp-witness-rulesp)
+                              state)
+  :guard-hints (("goal" :in-theory (enable pseudo-term-listp)))
+  :returns (actions wcp-lit-actions-listp)
+  (if (atom lits)
+      nil
+    (cons (wcp-lit-actions-for-lit (car lits) examples witness-rules state)
+          (wcp-actions-for-lits (cdr lits) examples witness-rules state)))
+  ///
+  (defthm len-of-wcp-actions-for-lits
+    (equal (len (wcp-actions-for-lits lits examples witness-rules state))
+           (len lits))))
+
+(define wcp-hint-for-clause ((clause pseudo-term-listp)
+                             (witness-rules wcp-witness-rulesp)
+                             (inst-rules wcp-instance-rulesp)
+                             (templates wcp-templatesp)
+                             state)
+  :returns (actions wcp-lit-actions-listp)
+  ;; There is a bunch of redundant work here -- we'll end up computing the
+  ;; witness rule unifications for successful rule applications a total of 4
+  ;; times apiece, three here and one in witness-cp.  Well... optimizations are
+  ;; possible, but this is pretty nice and clean.
+  (b* ((witness-only-actions (wcp-actions-for-lits clause nil witness-rules state))
+       ((mv witness-extended-clause ?gen-alist)
+        (wcp-clause-apply-actions clause witness-only-actions state))
+       (examples (wcp-collect-examples-list
+                  (wcp-beta-reduce-list witness-extended-clause)
+                  templates inst-rules nil state)))
+    (wcp-actions-for-lits clause examples witness-rules state))
+  ///
+  (defthm len-of-wcp-hint-for-clause
+    (equal (len (wcp-hint-for-clause clause witness-rules inst-rules templates state))
+           (len clause))))
+
+
+
+
+;;========================================================================
+;; Defwitness/definstantiate/defexample.
+;;========================================================================
+
+
 
 (defun wcp-translate (term ctx state)
   (declare (xargs :mode :program))
@@ -1751,24 +1249,37 @@
        ((er generalize-terms)
         (wcp-translate-lst (strip-cars generalize) 'defwitness state))
        (generalize (pairlis$ generalize-terms (strip-cdrs generalize)))
-       ((er &) (run-test-with-hint-replacement
-                `(implies ,predicate ,expr)
-                hints (cons 'defwitness name) state))
+
+       (thmname (intern-in-package-of-symbol
+                 (concatenate 
+                  'string (symbol-name name) "-WITNESS-RULE-CORRECT")
+                 name))
+       (obj (make-wcp-witness-rule :name name
+                                   :enabledp t
+                                   :term (dumb-negate-lit predicate)
+                                   :expr (dumb-negate-lit expr)
+                                   :restriction restriction
+                                   :theorem thmname
+                                   :generalize generalize))
+                              
        ;;                         `((prog2$ (cw "clause: ~x0~%" clause)
        ;;                                   '(:computed-hint-replacement
        ;;                                     :do-not '(preprocess simplify)))) nil nil))
        )
     (value
-     `(table witness-cp-witness-rules
-             ',name ',(list t
-                            (dumb-negate-lit predicate)
-                            (dumb-negate-lit expr)
-                            restriction hints generalize)))))
+     `(progn
+        (defthm ,thmname
+          (implies ,(dumb-negate-lit expr)
+                   ,(dumb-negate-lit predicate))
+          :hints ,hints
+          :rule-classes nil)
+        (table witness-cp-witness-rules
+               ',name ',obj)))))
 
-
-(defmacro defwitness (name &key predicate expr
-                           (restriction ''t)
-                           generalize hints)
+(defxdoc defwitness
+  :parents (witness-cp)
+  :short ""
+  :long 
   ":doc-section witness-cp
  Defwitness -- add a WITNESS-CP rule providing a witness for an
  existential-quantifier hypothesis (or universal-quantifier conclusion).~/
@@ -1802,10 +1313,14 @@
  replacement is sound (which is also done when the defwitness form is run).
 
  If a RESTRICTION is given, then this replacement will only take place when
- it evaluates to a non-nil value.~/"
+ it evaluates to a non-nil value.~/")
+
+
+(defmacro defwitness (name &key predicate expr
+                           (restriction ''t)
+                           generalize hints)
   `(make-event (defwitness-fn ',name ',predicate ',expr ',restriction
                  ',generalize ',hints state)))
-
 
 
 
@@ -1824,20 +1339,31 @@
         (wcp-translate expr 'definstantiate state))
        ((er restriction)
         (wcp-translate restriction 'definstantiate state))
-       ((er &) (run-test-with-hint-replacement
-                `(implies ,predicate ,expr)
-                hints (cons 'definstantiate name) state)))
-    (value
-     `(table witness-cp-instance-rules
-             ',name ',(list t
-                            (dumb-negate-lit predicate)
-                            vars
-                            (dumb-negate-lit expr)
-                            restriction hints)))))
 
-(defmacro definstantiate (name &key predicate vars expr
-                               (restriction ''t) hints)
-  ":doc-section witness-cp
+       (thmname (intern-in-package-of-symbol
+                 (concatenate 
+                  'string (symbol-name name) "-INSTANCE-RULE-CORRECT")
+                 name))
+       (obj (make-wcp-instance-rule :name name
+                                    :enabledp t
+                                    :pred (dumb-negate-lit predicate)
+                                    :vars vars
+                                    :expr (dumb-negate-lit expr)
+                                    :restriction restriction
+                                    :theorem thmname)))
+    (value
+     `(progn
+        (defthm ,thmname
+          (implies ,(dumb-negate-lit expr)
+                   ,(dumb-negate-lit predicate))
+          :hints ,hints
+          :rule-classes nil)
+        (table witness-cp-instance-rules ',name ',obj)))))
+
+(defxdoc definstantiate
+  :parents (witness-cp)
+  :short ""
+  :long ":doc-section witness-cp
  Definstantiate -- add a WITNESS-CP rule showing how to instantiate a
  universial-quantifier hyptothesis (or an existential-quantifier conclusion).~/
 
@@ -1870,10 +1396,141 @@
  sound (which is also done when the definstantiate form is run).
 
  If a RESTRICTION is given, then this replacement will only take place when
- it evaluates to a non-nil value.~/"
+ it evaluates to a non-nil value.~/")
+
+(defmacro definstantiate (name &key predicate vars expr
+                               (restriction ''t) hints)
+  
   `(make-event (definstantiate-fn
                  ',name ',predicate ',vars ',expr ',restriction
                  ',hints state)))
+
+
+(define missing-instance-rules ((instance-rules symbol-listp)
+                                (alist alistp))
+  (if (atom instance-rules)
+      nil
+    (if (assoc (car instance-rules) alist)
+        (missing-instance-rules (cdr instance-rules) alist)
+      (cons (car instance-rules)
+            (missing-instance-rules (cdr instance-rules) alist)))))
+
+
+(defun wrong-arity-instance-rules (arity instance-rules alist)
+  (declare (xargs :mode :program))
+  (if (atom instance-rules)
+      nil
+    (if (= (len (wcp-instance-rule->vars (cdr (assoc (car instance-rules) alist)))) arity)
+        (wrong-arity-instance-rules arity (cdr instance-rules) alist)
+      (cons (car instance-rules)
+            (wrong-arity-instance-rules arity (cdr instance-rules) alist)))))
+
+(defun defexample-fn (name pattern templates instance-rules restriction
+                           state)
+  (declare (Xargs :mode :program :stobjs state))
+  (b* (((when (not pattern))
+        (mv "DEFEXAMPLE: Must supply a :PATTERN.~%" nil state))
+       ((when (not templates))
+        (mv "DEFEXAMPLE: Must supply :TEMPLATES.~%" nil state))
+       ((when (not instance-rules))
+        (mv "DEFEXAMPLE: Must supply an :INSTANCE-RULENAME.~%" nil state))
+       (instance-rule-alist (table-alist 'witness-cp-instance-rules
+                                         (w state)))
+       (missing-rules (missing-instance-rules instance-rules instance-rule-alist))
+       ((when missing-rules)
+        (mv (msg "DEFEXAMPLE: The following instance rules do not exist: ~x0~%"
+                 missing-rules)
+            nil state))
+       (nvars (len templates))
+       (bad-rules (wrong-arity-instance-rules nvars instance-rules instance-rule-alist))
+       ((when bad-rules)
+        (mv (msg "DEFEXAMPLE: The following instance rules do not have the
+right number of free variables (~x0): ~x1~%"
+                 nvars bad-rules)
+            nil state))
+       ((er pattern)
+        (wcp-translate pattern 'defexample state))
+       ((er restriction)
+        (wcp-translate restriction 'defexample state))
+       ((er templates)
+        (wcp-translate-lst templates 'defexample state))
+       (obj (make-wcp-template :name name
+                               :enabledp t
+                               :pat pattern
+                               :templ templates
+                               :rulenames instance-rules
+                               :restriction restriction)))
+    (value
+     `(table witness-cp-example-templates
+             ',name ',obj))))
+
+(defxdoc defexample
+  :parents (witness-cp)
+  :short ""
+  :long 
+  ":doc-section witness-cp
+Defexample -- tell witness-cp how to instantiate the free variables of
+definstantiate rules~/
+
+Example:
+~bv[]
+ (defexample set-reasoning-member-template
+   :pattern (member-equal k y)
+   :templates (k)
+   :instance-rules
+   (subsetp-equal-instancing
+    intersectp-equal-instancing
+    set-equiv-instancing
+    set-consp-instancing))
+~ev[]
+
+Additional arguments:
+  :restriction term
+ where term may have free variables present in pattern as well as WORLD,
+  :instance-rulename rule
+ may be used instead of :instance-rules when there is only one rule.
+
+Meaning: Find terms of the form ~c[(member-equal k y)] throughout the clause,
+and for each such ~c[k], for any match of one of the instance-rules listed, add
+an instance using that ~c[k].  For example, if we have a hypothesis
+~c[(subsetp-equal a b)] and terms
+~bv[]
+ (member-equal (foo x) (bar y))
+ (member-equal q a)
+~ev[]
+present somewhere in the clause, then this rule along with the
+subsetp-equal-instancing rule will cause the following hyps to be added:
+~bv[]
+ (implies (member-equal (foo x) a)
+          (member-equal (bar x) a))
+ (implies (member-equal q a)
+          (member-equal q b)).
+~ev[]
+
+If a :restriction is present, then the rule only applies to occurrences of
+pattern for which the restriction evaluates to non-nil.~/~/")
+
+(defmacro defexample (name &key pattern templates instance-rulename
+                           instance-rules
+                           (restriction ''t))
+  `(make-event
+    (defexample-fn ',name ',pattern ',templates
+      ',(if instance-rulename (list instance-rulename) instance-rules)
+      ',restriction state)))
+       
+                                           
+
+
+
+
+
+
+
+
+
+
+
+
 
 
 (defun quantexpr-bindings-to-generalize (bindings)
@@ -1886,14 +1543,14 @@
 (defun defquantexpr-fn (name predicate quantifier expr witnesses
                              instance-restriction witness-restriction
                              instance-hints witness-hints
-                             witness-rulename instance-rulename
+                             wcp-witness-rulename instance-rulename
                              generalize in-package-of)
   (b* ((in-package-of (or in-package-of name))
        ((unless (member quantifier '(:forall :exists)))
         (er hard? 'defquantexpr
             "Quantifier argument must be either :FORALL or :EXISTS~%"))
-       (witness-rulename
-        (or witness-rulename
+       (wcp-witness-rulename
+        (or wcp-witness-rulename
             (intern-in-package-of-symbol
              (concatenate 'string (symbol-name name) "-WITNESSING")
              in-package-of)))
@@ -1914,7 +1571,7 @@
               `(let ,witnesses ,expr)
               `(not ,expr))))
        (generalize-alist (quantexpr-bindings-to-generalize witnesses)))
-    `(progn (defwitness ,witness-rulename
+    `(progn (defwitness ,wcp-witness-rulename
               :predicate ,witness-pred
               :expr ,witness-expr
               :hints ,witness-hints
@@ -1927,17 +1584,11 @@
               :hints ,instance-hints
               :restriction ,instance-restriction))))
 
-(defmacro defquantexpr (name &key predicate
-                             (quantifier ':forall)
-                             expr witnesses
-                             (instance-restriction ''t)
-                             (witness-restriction ''t)
-                             instance-hints witness-hints
-                             witness-rulename
-                             instance-rulename
-                             in-package-of
-                             (generalize 't))
-  ":doc-section witness-cp
+
+(defxdoc defquantexpr
+  :parents (witness-cp)
+  :short ""
+  :long ":doc-section witness-cp
  Defquantexpr -- shortcut to perform both a DEFWITNESS and DEFINSTANTIATE~/
 
  Usage:
@@ -1955,7 +1606,7 @@
  defwitness and definstantiate rules produced are generated from the name
  (first argument) of the defquantexpr form; in this case they are
  subsetp-witnessing and subsetp-equal-instancing.  Keyword arguments
- witness-rulename and instance-rulename may be provided to override these
+ wcp-witness-rulename and instance-rulename may be provided to override these
  defaults.
 
  Witness-hints and instance-hints are the hints passed to the two forms.
@@ -2020,10 +1671,22 @@
           (member-equal k y))).\"
 ~ev[]~/
 
-"
+")
+
+(defmacro defquantexpr (name &key predicate
+                             (quantifier ':forall)
+                             expr witnesses
+                             (instance-restriction ''t)
+                             (witness-restriction ''t)
+                             instance-hints witness-hints
+                             wcp-witness-rulename
+                             instance-rulename
+                             in-package-of
+                             (generalize 't))
+  
   (defquantexpr-fn name predicate quantifier expr witnesses
      instance-restriction witness-restriction
-     instance-hints witness-hints witness-rulename instance-rulename generalize in-package-of))
+     instance-hints witness-hints wcp-witness-rulename instance-rulename generalize in-package-of))
 
 
 
@@ -2031,160 +1694,60 @@
 
 
 
-(defun missing-instance-rules (instance-rules alist)
-  (declare (xargs :guard (and (alistp alist)
-                              (symbol-listp instance-rules))))
-  (if (atom instance-rules)
-      nil
-    (if (assoc (car instance-rules) alist)
-        (missing-instance-rules (cdr instance-rules) alist)
-      (cons (car instance-rules)
-            (missing-instance-rules (cdr instance-rules) alist)))))
 
 
-(defun wrong-arity-instance-rules (arity instance-rules alist)
-  (declare (xargs :mode :program))
-  (if (atom instance-rules)
-      nil
-    (if (= (len (nth 3 (assoc (car instance-rules) alist))) arity)
-        (wrong-arity-instance-rules arity (cdr instance-rules) alist)
-      (cons (car instance-rules)
-            (wrong-arity-instance-rules arity (cdr instance-rules) alist)))))
-
-(defun defexample-fn (name pattern templates instance-rules restriction
-                           state)
-  (declare (Xargs :mode :program :stobjs state))
-  (b* (((when (not pattern))
-        (mv "DEFEXAMPLE: Must supply a :PATTERN.~%" nil state))
-       ((when (not templates))
-        (mv "DEFEXAMPLE: Must supply :TEMPLATES.~%" nil state))
-       ((when (not instance-rules))
-        (mv "DEFEXAMPLE: Must supply an :INSTANCE-RULENAME.~%" nil state))
-       (instance-rule-alist (table-alist 'witness-cp-instance-rules
-                                         (w state)))
-       (missing-rules (missing-instance-rules instance-rules instance-rule-alist))
-       ((when missing-rules)
-        (mv (msg "DEFEXAMPLE: The following instance rules do not exist: ~x0~%"
-                 missing-rules)
-            nil state))
-       (nvars (len templates))
-       (bad-rules (wrong-arity-instance-rules nvars instance-rules instance-rule-alist))
-       ((when bad-rules)
-        (mv (msg "DEFEXAMPLE: The following instance rules do not have the
-right number of free variables (~x0): ~x1~%"
-                 nvars bad-rules)
-            nil state))
-       ((er pattern)
-        (wcp-translate pattern 'defexample state))
-       ((er restriction)
-        (wcp-translate restriction 'defexample state))
-       ((er templates)
-        (wcp-translate-lst templates 'defexample state)))
-    (value
-     `(table witness-cp-example-templates
-             ',name ',(list t pattern templates instance-rules restriction)))))
-
-(defmacro defexample (name &key pattern templates instance-rulename
-                           instance-rules
-                           (restriction ''t))
-  ":doc-section witness-cp
-Defexample -- tell witness-cp how to instantiate the free variables of
-definstantiate rules~/
-
-Example:
-~bv[]
- (defexample set-reasoning-member-template
-   :pattern (member-equal k y)
-   :templates (k)
-   :instance-rules
-   (subsetp-equal-instancing
-    intersectp-equal-instancing
-    set-equiv-instancing
-    set-consp-instancing))
-~ev[]
-
-Additional arguments:
-  :restriction term
- where term may have free variables present in pattern as well as WORLD,
-  :instance-rulename rule
- may be used instead of :instance-rules when there is only one rule.
-
-Meaning: Find terms of the form ~c[(member-equal k y)] throughout the clause,
-and for each such ~c[k], for any match of one of the instance-rules listed, add
-an instance using that ~c[k].  For example, if we have a hypothesis
-~c[(subsetp-equal a b)] and terms
-~bv[]
- (member-equal (foo x) (bar y))
- (member-equal q a)
-~ev[]
-present somewhere in the clause, then this rule along with the
-subsetp-equal-instancing rule will cause the following hyps to be added:
-~bv[]
- (implies (member-equal (foo x) a)
-          (member-equal (bar x) a))
- (implies (member-equal q a)
-          (member-equal q b)).
-~ev[]
-
-If a :restriction is present, then the rule only applies to occurrences of
-pattern for which the restriction evaluates to non-nil.~/~/"
-  `(make-event
-    (defexample-fn ',name ',pattern ',templates
-      ',(if instance-rulename (list instance-rulename) instance-rules)
-      ',restriction state)))
-
-
-
-(defun look-up-witness-rules (rules table)
+(defun look-up-wcp-witness-rules (rules table)
   (if (atom rules)
       (mv nil nil)
-    (b* (((mv rest missing) (look-up-witness-rules (cdr rules) table))
+    (b* (((mv rest missing) (look-up-wcp-witness-rules (cdr rules) table))
          (look (assoc (car rules) table)))
       (if look
           (mv (cons look rest) missing)
         (mv rest (cons (car rules) missing))))))
 
 
-;; (defun def-witness-ruleset-fn (name witness-names instance-names
+;; (defun def-wcp-witness-ruleset-fn (name witness-names instance-names
 ;;                                     example-names state)
-;;   (b* (((mv witness-rules missing)
-;;         (look-up-witness-rules
+;;   (b* (((mv wcp-witness-rules missing)
+;;         (look-up-wcp-witness-rules
 ;;          witness-names
 ;;          (table-alist 'witness-cp-witness-rules (w state))))
 ;;        ((when missing)
-;;         (mv (msg "DEF-WITNESS-RULESET: Witness ~s0 not found: ~x1~%"
+;;         (mv (msg "DEF-WCP-WITNESS-RULESET: Witness ~s0 not found: ~x1~%"
 ;;                  (if (consp (cdr missing)) "rules" "rule")
 ;;                  missing)
 ;;             nil state))
 ;;        ((mv instance-rules missing)
-;;         (look-up-witness-rules
+;;         (look-up-wcp-witness-rules
 ;;          instance-names
 ;;          (table-alist 'witness-cp-instance-rules (w state))))
 ;;        ((when missing)
-;;         (mv (msg "DEF-WITNESS-RULESET: Instance ~s0 not found: ~x1~%"
+;;         (mv (msg "DEF-WCP-WITNESS-RULESET: Instance ~s0 not found: ~x1~%"
 ;;                  (if (consp (cdr missing)) "rules" "rule")
 ;;                  missing)
 ;;             nil state))
 ;;        ((mv example-templates missing)
-;;         (look-up-witness-rules
+;;         (look-up-wcp-witness-rules
 ;;          example-names
 ;;          (table-alist 'witness-cp-example-templates (w state))))
 ;;        ((when missing)
-;;         (mv (msg "DEF-WITNESS-RULESET: Example ~s0 not found: ~x1~%"
+;;         (mv (msg "DEF-WCP-WITNESS-RULESET: Example ~s0 not found: ~x1~%"
 ;;                  (if (consp (cdr missing)) "templates" "template")
 ;;                  missing)
 ;;             nil state)))
 ;;     (value `(table witness-cp-rulesets ',name
-;;                    ',(list witness-rules
+;;                    ',(list wcp-witness-rules
 ;;                            example-templates
 ;;                            instance-rules)))))
 
-(defmacro def-witness-ruleset (name rules)
-  ":doc-section witness-cp
-Def-witness-ruleset: name a set of witness-cp rules~/
+(defxdoc def-witness-ruleset
+  :parents (witness-cp)
+  :short ""
+  :long ":doc-section witness-cp
+def-witness-ruleset: name a set of witness-cp rules~/
 
 The WITNESS computed-hint macro takes a :ruleset argument that determines
-which witness-cp rules are allowed to fire.  Def-witness-ruleset allows
+which witness-cp rules are allowed to fire.  def-witness-ruleset allows
 one name to abbreviate several actual rules in this context.
 
 Usage:
@@ -2222,7 +1785,10 @@ Witness rules can also be enabled/disabled using ~il[witness-enable] and
 ~il[witness-disable]; these settings take effect when WITNESS is called without
 specifying a ruleset.  Ruleset names may be used in witness-enable and
 witness-disable just as they are used in the ruleset argument of WITNESS.
-~/~/"
+~/~/")
+
+(defmacro def-witness-ruleset (name rules)
+  
   `(table witness-cp-rulesets ',name ,rules))
 
 ;; (defun defquant-witness-binding1 (n qvars witness-expr)
@@ -2265,7 +1831,7 @@ witness-disable just as they are used in the ruleset argument of WITNESS.
 
 
 (defun defquant-fn (name vars quant-expr define
-                         witness-rulename
+                         wcp-witness-rulename
                          instance-rulename
                          doc
                          quant-ok
@@ -2318,25 +1884,14 @@ witness-disable just as they are used in the ruleset argument of WITNESS.
        :expr ,qexpr
        :witness-hints ('(:in-theory '(,name)))
        :instance-hints ('(:in-theory nil :use ,thm-name))
-       :witness-rulename ,witness-rulename
+       :wcp-witness-rulename ,wcp-witness-rulename
        :instance-rulename ,instance-rulename)
      (in-theory (disable ,name ,thm-name)))))
 
-
-(defmacro defquant (name vars quant-expr &key
-                         (define 't)
-                         witness-rulename
-                         instance-rulename
-                         ;; defun-sk args
-                         doc
-                         quant-ok
-                         skolem-name
-                         thm-name
-                         rewrite
-                         strengthen
-                         in-package-of
-                         (witness-dcls '((DECLARE (XARGS :NON-EXECUTABLE T)))))
-  ":doc-section witness-cp
+(defxdoc defquant
+  :parents (witness-cp)
+  :short ""
+  :long ":doc-section witness-cp
 Defquant -- define a quantified function and corresponding witness-cp rules~/
 
 Defquant introduces a quantified function using ~il[defun-sk] and subsequently
@@ -2350,11 +1905,27 @@ additional keywords:
   :define -- default t, use nil to skip the defun-sk step (useful if it
        has already been done)
 
-  :witness-rulename, :instance-rulename --
+  :wcp-witness-rulename, :instance-rulename --
      name the generated witness and instance rules.  The defaults are
-     name-witnessing and name-instancing.~/~/"
+     name-witnessing and name-instancing.~/~/")
 
-  (defquant-fn name vars quant-expr define witness-rulename instance-rulename
+
+(defmacro defquant (name vars quant-expr &key
+                         (define 't)
+                         wcp-witness-rulename
+                         instance-rulename
+                         ;; defun-sk args
+                         doc
+                         quant-ok
+                         skolem-name
+                         thm-name
+                         rewrite
+                         strengthen
+                         in-package-of
+                         (witness-dcls '((DECLARE (XARGS :NON-EXECUTABLE T)))))
+  
+
+  (defquant-fn name vars quant-expr define wcp-witness-rulename instance-rulename
     doc
     quant-ok
     skolem-name
@@ -2365,7 +1936,7 @@ additional keywords:
     in-package-of))
 
 
-(defun witness-rule-e/d-event (rulename tablename enablep world)
+(defun wcp-witness-rule-e/d-event (rulename tablename enablep world)
   (b* ((al (table-alist tablename world))
        (look (assoc rulename al)))
     (and look
@@ -2387,7 +1958,7 @@ additional keywords:
 (defun instance-rules-for-examples (example-templates)
   (if (atom example-templates)
       nil
-    (append (nth 4 (car example-templates))
+    (append (wcp-template->rulenames (car example-templates))
             (instance-rules-for-examples (cdr example-templates)))))
 
 
@@ -2396,22 +1967,22 @@ additional keywords:
    (declare (xargs :mode :program))
    ;; Union together the rules mentioned as well as the rules within the
    ;; rulesets.
-   (b* (((mv witness-rules instance-rules example-templates rest)
+   (b* (((mv wcp-witness-rules instance-rules example-templates rest)
          (witness-expand-ruleset-names names world))
-        ((mv witness-rules1 &)
-         (look-up-witness-rules rest (table-alist 'witness-cp-witness-rules world)))
+        ((mv wcp-witness-rules1 &)
+         (look-up-wcp-witness-rules rest (table-alist 'witness-cp-witness-rules world)))
         ((mv example-templates1 &)
-         (look-up-witness-rules rest (table-alist 'witness-cp-example-templates
+         (look-up-wcp-witness-rules rest (table-alist 'witness-cp-example-templates
                                                   world)))
         (example-templates1 (remove-dups-assoc example-templates1))
         ((mv instance-rules1 &)
-         (look-up-witness-rules (instance-rules-for-examples example-templates1)
+         (look-up-wcp-witness-rules (instance-rules-for-examples example-templates1)
                                 (table-alist 'witness-cp-instance-rules
                                              world)))
         ((mv instance-rules2 &)
-         (look-up-witness-rules rest (table-alist 'witness-cp-instance-rules
+         (look-up-wcp-witness-rules rest (table-alist 'witness-cp-instance-rules
                                                   world))))
-     (mv (union-assoc (remove-dups-assoc witness-rules1) witness-rules)
+     (mv (union-assoc (remove-dups-assoc wcp-witness-rules1) wcp-witness-rules)
          (union-assoc (remove-dups-assoc instance-rules1)
                       (union-assoc (remove-dups-assoc instance-rules2)
                                    instance-rules))
@@ -2420,17 +1991,17 @@ additional keywords:
  (defun witness-expand-ruleset-names (names world)
    (if (atom names)
        (mv nil nil nil nil)
-     (b* (((mv witness-rules instance-rules example-templates rest)
+     (b* (((mv wcp-witness-rules instance-rules example-templates rest)
            (witness-expand-ruleset-names (cdr names) world))
           (ruleset-look
            (assoc (car names)
                   (table-alist 'witness-cp-rulesets world)))
           ((when (not ruleset-look))
-           (mv witness-rules instance-rules example-templates
+           (mv wcp-witness-rules instance-rules example-templates
                (cons (car names) rest)))
-          ((mv witness-rules1 instance-rules1 example-templates1)
+          ((mv wcp-witness-rules1 instance-rules1 example-templates1)
            (witness-expand-ruleset (cdr ruleset-look) world)))
-       (mv (union-assoc witness-rules1 witness-rules)
+       (mv (union-assoc wcp-witness-rules1 wcp-witness-rules)
            (union-assoc instance-rules1 instance-rules)
            (union-assoc example-templates1 example-templates)
            rest)))))
@@ -2438,7 +2009,7 @@ additional keywords:
 (defun witness-e/d-events (names tablename enablep world)
   (if (atom names)
       nil
-    (append (witness-rule-e/d-event (car names) tablename enablep world)
+    (append (wcp-witness-rule-e/d-event (car names) tablename enablep world)
             (witness-e/d-events (cdr names) tablename enablep world))))
 
 (defun witness-e/d-ruleset-fn (names enablep world)
@@ -2451,46 +2022,21 @@ additional keywords:
          ,@(witness-e/d-events (strip-cars i) 'witness-cp-instance-rules enablep world)
          . ,(witness-e/d-events (strip-cars e) 'witness-cp-example-templates enablep world)))))
 
+
+
+
 (defmacro witness-enable (&rest names)
-  ":doc-section witness-cp
- Witness-enable -- enable some witness-cp rules~/
-
- Usage:
-~bv[]
- (witness-enable name1 name2 ...)
-~ev[]
-
- Sets the witness-cp rules name1, name2... to be enabled by default.
-When name1 is the name of a witness-ruleset rather than a rule, all rules in
-the ruleset are set enabled.
-
-The enabled/disabled setting of a witness-cp rule takes effect only when
-WITNESS is called with no :ruleset argument; otherwise, the ruleset specified
-ignores the enabled/disabled status.~/~/"
   `(make-event (witness-e/d-ruleset-fn ',names t (w state))))
 
 (defmacro witness-disable (&rest names)
-  ":doc-section witness-cp
- Witness-disable -- disable some witness-cp rules~/
-
- Usage:
-~bv[]
- (witness-disable name1 name2 ...)
-~ev[]
-
- Sets the witness-cp rules name1, name2... to be disabled by default.
-When name1 is the name of a witness-ruleset rather than a rule, all rules in
-the ruleset are set disabled.
-
-The enabled/disabled setting of a witness-cp rule takes effect only when
-WITNESS is called with no :ruleset argument; otherwise, the ruleset specified
-ignores the enabled/disabled status.~/~/"
   `(make-event (witness-e/d-ruleset-fn ',names nil (w state))))
 
 
 
-(defmacro witness (&key ruleset (generalize 't) examples)
-  ":doc-section witness-cp
+(defxdoc witness
+  :parents (witness-cp)
+  :short "Computed hint for calling the witness clause processor"
+  :long ":doc-section witness-cp
 Witness -- computed-hint that runs witness-cp~/
 
 Usage:
@@ -2515,28 +2061,30 @@ universally-quantified hyps in a particular way on a one-off basis; this may be
 done using the :examples field.  Each inst-rulename must be the name of a
 definstantiate rule, and the terms following it correspond to that rule's :vars
  (in partiular, the list of terms must be the same length as the :vars of the
-rule).~/~/"
+rule).~/~/")
+
+
+(defmacro witness (&key ruleset)
   `(and stable-under-simplificationp
         (b* ((ruleset ',ruleset)
-             (examples ',examples)
-             (rules/user-examples
+             ((mv w i e)
               (if ruleset
-                  (mv-let (w i e)
-                    (witness-expand-ruleset
-                     (if (atom ruleset) (list ruleset) ruleset)
-                     world)
-                    (list w e i examples))
-                (list (table-alist 'witness-cp-witness-rules world)
-                      (table-alist 'witness-cp-example-templates
-                                   world)
-                      (table-alist 'witness-cp-instance-rules
-                                   world)
-                      examples)))
-               (hints (cons ',generalize rules/user-examples)))
-          `(:computed-hint-replacement
-            ((use-these-hints-hint clause))
-            :clause-processor
-            (witness-cp clause ',hints state)))))
+                  (witness-expand-ruleset
+                   (if (atom ruleset) (list ruleset) ruleset)
+                   world)
+                (mv (table-alist 'witness-cp-witness-rules world)
+                    (table-alist 'witness-cp-instance-rules
+                                 world)
+                    (table-alist 'witness-cp-example-templates
+                                 world))))
+             (hint (wcp-hint-for-clause
+                    clause
+                    (strip-cdrs w)
+                    (strip-cdrs i)
+                    (strip-cdrs e) state)))
+          `(:clause-processor
+            (witness-cp clause ',hint state)))))
+
 
 
 
